vminus/CFG.v
@@ -1,0 +1,189 @@
+Require Import Arith.
+Require Import Vminus.Util.
+Require Import Vminus.Classes.
+Require Import Vminus.Vminus.
+
+(* ################################################################# *)
+(** * CFG: Control-flow Graphs *)
+
+(** Vminus programs are structured into _control-flow graphs_
+    (CFG), which, conceptually, are graphs whose _nodes_ are
+    instructions and whose _edges_ are determined by the control
+    structure of the program.
+
+    To characterize this structure abstractly, we define a notion of
+    _program point_ [pc], which is a location of an instruction in the
+    control-flow graph (i.e. each program point is a node of the
+    graph).
+
+    The program points are themselves organized into _basic blocks_.
+    A basic block consists of a non-empty sequence of program points 
+    ending in a terminator instruction.
+ *)
+
+(* ################################################################# *)
+(** * Program points *)
+
+(** Program points (a.k.a. "program counters").
+    Concretely, a [pc] is given by a block label and offset.
+
+    (We could make this more abstract, but this is a simple, easy-to-work with definition.)
+ *)
+
+Definition pc := (lbl * nat)%type.
+
+(** Each [pc] has a label *)
+
+Definition lbl_of : pc -> lbl       := @fst _ _.
+
+(** Increment a [pc] _within_ a block. *)
+
+Definition incr_pc (p:pc) : pc :=
+  let (l, n) := p in (l, S n).
+
+(** (Total) Ordering on [pc]s within the same block *)
+
+Inductive le_pc : pc -> pc -> Prop :=
+| let_pc_intro : forall l n1 n2,
+    n1 <= n2 -> le_pc (l, n1) (l, n2).
+
+Definition lt_pc (p1 p2:pc) : Prop :=
+  le_pc p1 (incr_pc p2).
+
+Definition eq_dec_pc: forall p1 p2: pc, {p1 = p2} + {~(p1 = p2)}.
+Proof.
+  intros (lbl1, offset1) (lbl2, offset2).
+  destruct (eq_dec_lbl lbl1 lbl2) as [lbl_eq | lbl_neq];
+    try solve [right; intros H; inversion H;
+               exfalso; apply lbl_neq; trivial];
+  destruct (Nat.eq_dec offset1 offset2) as [offset_eq | offset_neq];
+    try solve [right; intros H; inversion H; apply offset_neq; trivial];
+    left; subst; reflexivity.
+Defined.
+
+(** The entry point of a block is offset [0]. *)
+
+Definition block_entry (l:lbl) : pc := (l, 0).
+Definition entry_of_pc (p:pc)  : pc := block_entry (fst p).
+
+
+(**  ------------------------------------------------------------------------- *)
+(* ################################################################# *)
+(** * Interface for syntactically well-formed CFGs *)
+
+(** Given the abstract characterization of program points, we need to
+    relate them to the control-flow instructions of the program's CFG.
+    We do this via a collection of well-formedness predicates that
+    ensure that each program point maps to a single instruction and
+    that the instruction defines a unique local identifier.  (Thus
+    satisfying the 'single static assignment' part of the SSA
+    representation.)
+ *)
+
+(** 
+    In this interface, we establish the basic syntactic properties of 
+    control-flow-graphs:
+
+    - A CFG [g] is a (partial) function from program points to instructions.
+    - Each program point belongs to a basic block.
+    - Each basic block is non-empty
+    - Each basic block consists of a contiguous sequence of program points,
+      ending in a terminator.
+
+    We will impose stronger well-formedness constraints (i.e. the SSA 
+    conditions) on CFGs later.
+*)
+
+
+Module Type CFG.
+  Parameter t : Type.
+  Local Notation cfg := t.
+
+(* ----------------------------------------------------------------- *)
+(** *** Basic parameters of the model *)
+
+  (** Well-formed control-flow-graphs. *)
+
+  Parameter wf_cfg : cfg -> Prop.
+
+  (** Well-formed program points. *)
+
+  Parameter wf_pc : cfg -> pc -> Prop.
+
+  (** *** *)
+
+  (** The entry block of the control-flow graph. *)
+
+  Parameter entry_block : cfg -> lbl.
+
+  (** Is the program point a block terminator? *)
+
+  Parameter tmn_pc : cfg -> pc -> Prop.
+
+  (** *** Program point properties *)
+
+  (** Program points are associated with unique instructions. *)
+
+  (** Relational specification: *)
+
+  Parameter insn_at_pc : cfg -> pc -> insn -> Prop.
+
+  Axiom insn_at_pc_func : forall g, wf_cfg g ->
+    functional (insn_at_pc g).
+  
+  (** Executable specification: *)
+  
+  Parameter fetch : cfg -> pc -> option insn.
+
+  (** Correspondence of the two specs: *)
+  
+  Axiom insn_at_pc_fetch :
+    forall g pc i, wf_cfg g ->
+              insn_at_pc g pc i <-> fetch g pc = Some i.
+
+  (** Each [pc] defines a unique [uid] *)
+  
+  Definition uid_at_pc (g:cfg) (p:pc) (uid:uid) : Prop :=
+    exists c, insn_at_pc g p (uid, c).
+
+  Axiom uid_at_pc_inj : forall g, wf_cfg g ->
+                             injective (uid_at_pc g).
+
+  Axiom uid_at_pc_func : forall g, wf_cfg g ->
+    functional (uid_at_pc g).
+  
+  Axiom pc_at_uid_inj : forall g, wf_cfg g ->
+                             injective (fun x p => uid_at_pc g p x).
+
+  Axiom eq_pc_uid : forall g pc id1 id2 c1 c2,
+    wf_cfg g ->
+    insn_at_pc g pc (id1, c1) ->
+    insn_at_pc g pc (id2, c2) ->
+    id1 = id2.
+
+  
+  (** If [g] is well-formed, each of its program points
+      maps to an instruction. *)  
+  
+  Axiom wf_pc_insn : forall g, wf_cfg g ->
+    forall p, wf_pc g p -> exists i, insn_at_pc g p i.
+
+  
+  (** *** Block properties *)
+
+  (** There is an instruction in the entry block. *)
+
+  Axiom wf_entry : forall g, wf_cfg g ->
+    wf_pc g (block_entry (entry_block g)).
+
+  (** Every block has a terminator. *)
+
+  Axiom wf_pc_tmn : forall g, wf_cfg g ->
+    forall p, wf_pc g p -> exists p', tmn_pc g p' /\ le_pc p p'.
+
+  (** There are no "gaps" in the pc labels. *)
+
+  Axiom wf_pc_le_tmn : forall g, wf_cfg g ->
+    forall p', tmn_pc g p' -> forall p, le_pc p p' -> wf_pc g p.
+
+End CFG.
