vminus/Compiler.v
@@ -1,0 +1,172 @@
+(* -------------------------------------------------------------------------- *
+ *                     Vellvm - the Verified LLVM project                     *
+ *                                                                            *
+ *     Copyright (c) 2017 Steve Zdancewic <stevez@cis.upenn.edu>              *
+ *                                                                            *
+ *   This file is distributed under the terms of the GNU General Public       *
+ *   License as published by the Free Software Foundation, either version     *
+ *   3 of the License, or (at your option) any later version.                 *
+ ---------------------------------------------------------------------------- *)
+
+
+(* ################################################################# *)
+(** * Imp to Vminus Compiler *)
+
+(** Imports, instantiated with the list implementation of 
+    control-flow graphs. *)
+
+Require Import List.
+Import ListNotations.
+
+Require Import Vminus.Classes Vminus.Imp Vminus.Vminus.
+Require Import Vminus.CFG.
+Require Import Vminus.ListCFG.
+Import ListCFG.
+
+(* ################################################################# *)
+(** * Compiling Expressions *)
+
+(** Compilation context for expressions.  The state monad keeps track
+    of the list of generated uids so that we can generate fresh names. *)
+
+Notation ectmon := (ST (list uid)).
+
+(** Generate a fresh uid. *)
+
+Definition fresh : ectmon uid :=
+  fun is =>
+  let i := Uid.fresh is in
+  (i::is, i).
+
+Definition strun {A:Set} (m:ectmon A) (l:list uid) : A :=
+  snd (m l).
+
+(* ================================================================= *)
+(** ** Compiling binops. *)
+
+(** Compile a general binary operation. *)
+
+(*! Section comp_bop *)
+
+Definition comp_bop (b:bop) (e1 e2: ectmon (val * list insn)) : ectmon (val * list insn) :=
+  '(v1, c1) <- e1;
+  '(v2, c2) <- e2;
+  'r <- fresh; 
+  mret (val_uid r, (c1 ++ c2 ++ [(r, cmd_bop b v1 v2)])).
+
+(** Compile an arithmetic expression. *)
+
+(*! Section comp_aexp *)
+
+Fixpoint comp_aexp (a:aexp) : ectmon (val * list insn) :=
+  match a with
+    | ANum n => mret (val_nat n, [])
+    | AId i => 'r <- fresh; mret (val_uid r, [(r, cmd_load i)])
+    | APlus a1 a2 => (*!*)comp_bop bop_add (comp_aexp a1) (comp_aexp a2)
+                    (*! comp_bop bop_add (comp_aexp a1) (comp_aexp a1) *)
+    | AMinus a1 a2 => (*! *) comp_bop bop_sub (comp_aexp a1) (comp_aexp a2)
+                     (*! comp_bop bop_sub (comp_aexp a1) (comp_aexp a1) *)
+    | AMult a1 a2 => (*! *) comp_bop bop_mul (comp_aexp a1) (comp_aexp a2)
+                    (*! comp_bop bop_mul (comp_aexp a1) (comp_aexp a1) *)
+  end.
+
+(* ================================================================= *)
+(** ** Compiling boolean expressions. *)
+
+(*! Section comp_bexp *)
+Fixpoint comp_bexp (b:bexp) : ectmon (val * list insn) :=
+  match b with
+    | BTrue => (*! *) mret (val_nat 1, []) (*! ret (val_nat 0, []) *)
+    | BFalse => mret (val_nat 0, [])
+    | BEq a1 a2 => comp_bop bop_eq (comp_aexp a1) (comp_aexp a2)
+    | BLe a1 a2 => (*! *) comp_bop bop_le (comp_aexp a1) (comp_aexp a2)
+                  (*! comp_bop bop_le (comp_aexp a1) (comp_aexp a1) *)
+    | BAnd b1 b2 => (*!*) comp_bop bop_and (comp_bexp b1) (comp_bexp b2)
+                   (*! comp_bop bop_and (comp_bexp b1) (comp_bexp b1) *)
+    | BNot b1 => (*!*) comp_bop bop_eq (comp_bexp b1) (mret (val_nat 0, []))
+                (*! comp_bop bop_eq (comp_bexp b1) (ret (val_nat 1, [])) *)
+  end.
+
+
+
+Definition comp_store (a:aexp) (v:addr) (lr:lbl) : ectmon (list insn) :=
+  'x <- fresh;
+  'y <- fresh;
+  '(i, is) <- comp_aexp a; 
+  mret (is ++ [ (x, cmd_store v i); 
+               (y, cmd_tmn (tmn_jmp lr)) ]).
+
+Definition comp_cond (b:bexp) (l1 l2:lbl) : ectmon (list insn) :=
+  '(v, is) <- comp_bexp b;
+  'x <- fresh;
+  mret (is ++ [ (x, cmd_tmn (tmn_cbr v l1 l2)) ] ).
+
+(* ================================================================= *)
+(* ** Compiling Commands *)
+
+(** State:
+    - list of used block labels
+    - list of used uids
+    - current cfg *)
+
+Definition cstate := (list lbl * list uid * list block)%type.
+Notation ctmon := (ST cstate).
+
+Definition fresh_lbl : ctmon lbl :=
+  fun cs =>
+  let '(ls, is, bs) := cs in
+  let l := Lbl.fresh ls in 
+  (l::ls, is, update bs l [], l).
+
+Definition raise_ectmon {T} (ec:ectmon T) : ctmon T :=
+  fun cs =>
+  let '(ls, is, cfg) := cs in
+  let (is', r) := ec is in
+  (ls, is', cfg, r).
+
+Definition add_insns (l:lbl) (b:list insn) : ctmon unit :=
+  fun cs =>
+  let '(ls, is, cfg) := cs in
+  (ls, is, update cfg l b, tt).
+
+(** The input [lr] is the label of the block to which
+    control should return after the command is done. 
+    The output is the label of the entry block for the
+    command. *)
+
+Fixpoint comp_com (c:Imp.com) (lr:lbl) : ctmon lbl :=
+  match c with
+    | CSkip => mret lr
+    | CAss i a => 
+        'l <- fresh_lbl;
+        'b <- raise_ectmon (comp_store a i lr);
+        '_ <- add_insns l b;
+        mret l
+    | CSeq c1 c2 =>
+        'l <- comp_com c2 lr; comp_com c1 l
+    | CIf b c1 c2 =>
+        'l1 <- comp_com c1 lr;
+        'l2 <- comp_com c2 lr;
+        'lh <- fresh_lbl;
+        'b  <- raise_ectmon (comp_cond b l1 l2);
+        '_  <- add_insns lh b;
+        mret lh
+    | CWhile b c => 
+        'lh <- fresh_lbl;
+        'lb <- comp_com c lh;
+        'b  <- raise_ectmon (comp_cond b lb lr);
+        '_  <- add_insns lh b;
+        mret lh
+  end.
+
+Definition comp_prog (c:com) : ctmon (lbl * lbl) :=
+  'r <- fresh_lbl;
+  'x <- raise_ectmon fresh;
+  '_ <- add_insns r [(x, cmd_tmn tmn_ret)];
+  'e <- comp_com c r;
+  mret (e, r).
+
+(* TODO: le is redundant ... fix up match_config *)
+Definition compile (c:com) : ListCFG.t * lbl * lbl :=
+  let '(_, _, bs, (le, lr)) := comp_prog c ([], [], []) in
+    ((le, bs), le, lr).
