vminus/CompilerProp.v
@@ -1,0 +1,977 @@
+Require Import FunctionalExtensionality. (* TODO: don't really need this *)
+Require Import List.
+Import ListNotations.
+Require Import RelationClasses.
+
+
+Require Import Vminus.Util Vminus.Classes.
+Require Import Vminus.Vminus.
+Require Import Vminus.CFG.
+Require Import Vminus.ListCFG.
+Require Import Vminus.Sequences.
+Require Import Vminus.VminusOpSem.
+Require Import Vminus.Imp.
+Require Import Vminus.Compiler.
+
+Import V.Opsem.
+
+
+Set Bullet Behavior "Strict Subproofs".
+Unset Printing Records.
+
+
+(* ################################################################# *)
+(** * To possibly refactor into CFGProp *)
+(* ================================================================= *)
+(** ** Correspondence between concrete and abstract CFGs. *)
+
+(** Asserts that the instruction sequence found at program point p in 
+    the control-flow graph g is exactly the list [is]. *)
+
+Fixpoint insns_at_pc (g:ListCFG.t) (p:pc) (is:list insn) : Prop := 
+  match is with
+    | nil => True
+    | i :: is' => ListCFG.insn_at_pc g p i /\ insns_at_pc g (incr_pc p) is'
+  end.
+
+(** Looking up the block labeled [l] in the concrete represenation
+    agrees with the declarative specification. *)
+
+Lemma cfg_insns_at : forall g l is e,
+  ListCFG.lookup g l = Some is ->
+  insns_at_pc (e, g) (block_entry l) is.
+Proof.
+  intros.
+  pose (k:=@nil insn). change is with (k ++ is) in H.
+  unfold block_entry. change 0 with (length k).
+  clearbody k. generalize dependent k.
+  induction is; intros. simpl; auto.
+    simpl. split. eexists. split.
+    unfold ListCFG.lookup in H.
+    apply assoc_in in H. simpl; eauto.
+    clear H. induction k; simpl; auto.
+    replace (S (length k)) with (length (k ++ [a])). apply IHis.
+      rewrite <- app_assoc. auto. rewrite app_length.
+      simpl. apply PeanoNat.Nat.add_1_r.
+Qed.
+
+(* ################################################################# *)
+(** * End refactoring *)
+
+
+(* ================================================================= *)
+(** ** Auxiliary definitions. *)
+
+Definition ids_preserved (cs:list uid) (st st':state) : Prop :=
+  forall uid n, In uid cs -> 
+    st_loc st uid = Some n -> st_loc st' uid = Some n.
+
+Definition good_return (cs:list uid) (v:val) : Prop :=
+  forall uid, v = val_uid uid -> In uid cs.
+
+Definition ctx_incr (cs cs':list uid) : Prop :=
+  forall uid, In uid cs -> In uid cs'.
+
+Instance ctx_incr_trans : Transitive ctx_incr.
+Proof. red; unfold ctx_incr; intuition. Qed.
+
+
+
+(* ################################################################# *)
+(** * Proofs start here; commented out because of QuickChick for now  *)
+Definition comp_correct (comp : ectmon (val * list insn))
+                        (eval : mem -> nat) : Prop :=
+  forall cs cs' g st is k v,
+  (cs', (v, is)) = comp cs ->
+  insns_at_pc g (st_pc st) (is ++ k) ->
+  exists st',
+    st_mem st' = st_mem st /\
+    insns_at_pc g (st_pc st') k /\
+    star (step g) st st' /\
+    ids_preserved cs st st' /\
+    good_return cs' v /\
+    ctx_incr cs cs' /\
+    eval_val (st_loc st') v = Some (eval (st_mem st)).
+
+Lemma comp_bop_correct : forall b comp1 comp2 eval1 eval2
+    (IHa1: comp_correct comp1 eval1)
+    (IHa2: comp_correct comp2 eval2),
+    comp_correct (comp_bop b comp1 comp2)
+                 (fun m => bop_denote b (eval1 m) (eval2 m)).
+Proof.
+  unfold comp_correct. 
+  intros b comp1 comp2 eval1 eval2.
+  intros until v. intros Hcomp Hinsns.
+
+  unfold comp_bop in Hcomp.
+  simpl in Hcomp.
+  destruct (comp1 cs) as [cs1 [rl1 rr1]] eqn:Hc1.
+  destruct (comp2 cs1) as [cs2 [rl2 rr2]] eqn:Hc2.
+  inversion Hcomp; clear Hcomp.
+
+  subst.
+  repeat rewrite <- app_assoc in Hinsns.
+  eelim IHa1; [| eauto ..]. 
+  intros st1 (Hinv1 & His1 & Hstep1 & Hpres1 & Hret1 & Hincr1 & Heval1).
+  eelim IHa2; [| eauto ..]. 
+  intros st2 (Hinv2 & His2 & Hstep2 & Hpres2 & Hret2 & Hincr2 & Heval2).
+  clear IHa1 IHa2.
+  
+  rename st2 into st2'; set (st2:=st2') in *; destruct st2'.
+  eexists {| st_pc  := incr_pc (st_pc st2);
+             st_loc := Locals.update (st_loc st2) (Uid.fresh cs2) _ |}. simpl.
+
+  (* exp_invar *)
+  split. transitivity (st_mem st1). transitivity (st_mem st2). reflexivity. auto.  apply Hinv1.
+
+  (* insns_at_pc *)
+  split. inversion His2; auto.
+
+  (* star (Opsem.step g) *)
+  split. eapply star_trans; eauto. eapply star_trans; eauto.
+    eapply star_one. eapply step_bop. inversion His2; eauto.  
+    unfold eval_bop. simpl in Heval2. rewrite Heval2. 
+    replace (eval_val st_loc0 _) with (Some (eval1 (st_mem st))).
+    reflexivity. symmetry. 
+
+    destruct rl1; auto. simpl. 
+    unfold good_return in *.
+    rename t into t0.
+    assert (In t0 cs1). apply Hret1; auto.
+    unfold ids_preserved in Hpres2.
+    apply Hpres2. auto. auto.
+
+  (* ids_preserved *)
+  split. red; simpl; intros. rewrite Locals.update_neq.
+  change st_loc0 with (st_loc st2).
+  apply Hpres2; auto. apply Hincr1, Hincr2 in H.
+  inversion Hc2. contradict H. rewrite <- H. apply Uid.fresh_not_in.
+
+  (* good_return *)
+  split. red. intros uid' Hid. injection Hid; inversion Hc2. left; auto.
+
+  (* ctx_incr *)
+  split. transitivity cs1; auto. transitivity cs2; auto. 
+  unfold ctx_incr. inversion Hc2; intros. right; auto.
+
+  (* eval_val *)
+  simpl. rewrite Locals.update_eq.
+  replace (st_mem st1) with (st_mem st). subst. reflexivity. 
+  inversion Hinv1; auto. reflexivity.
+Qed.
+
+
+Lemma comp_aexp_correct : forall (a:aexp),
+  comp_correct (comp_aexp a) (aeval a).
+Proof.
+  (* comp_bop_correct takes care of all the inductive cases *)
+  induction a; [ | | eapply comp_bop_correct; auto ..].
+
+  - (* Case "ANum". *)
+  unfold comp_correct; intros. inversion H; subst; clear H. 
+  exists st. repeat split; try red; auto using star_refl. discriminate.
+
+  - (* Case "AId". *)
+  unfold comp_correct. intros cs cs' g st is k v Hcomp Hinsns.
+  simpl in Hcomp. 
+  destruct (fresh cs) as [cs1 idr] eqn:Hc.
+  inversion Hcomp. clear Hcomp. subst.
+
+  rename st into st'. set (st := st'). destruct st'.
+  eexists {| st_pc := (incr_pc (st_pc st));
+             st_loc := Locals.update (st_loc st) idr _ |}. simpl.
+  split. reflexivity.
+  split. inversion Hinsns; auto.
+  split. apply star_one. apply step_load.
+  inversion Hinsns; eauto.
+  simpl in *.
+  unfold fresh in Hc. inversion Hc. apply H.
+  split. red; simpl; intros. rewrite Locals.update_neq; auto. 
+    inversion Hc. contradict H. rewrite <- H. apply Uid.fresh_not_in.
+  split. red. intros. inversion Hc. injection H; intro. subst idr uid. left; auto.
+  split. inversion Hc; red; intuition.
+  rewrite Locals.update_eq. reflexivity. inversion Hc. reflexivity.
+Qed.
+
+Local Hint Resolve comp_aexp_correct.
+
+Lemma comp_bexp_correct : forall (b:bexp),
+  comp_correct (comp_bexp b) (fun m => b2n (beval b m)).
+Proof.
+  induction b.
+
+  - (* Case "BTrue". *)
+  unfold comp_correct; intros. inversion H; subst; clear H. 
+  exists st; repeat split; try red; auto using star_refl. discriminate.
+
+  - (* Case "BFalse". *)
+  unfold comp_correct; intros. inversion H; subst; clear H. 
+  exists st; repeat split; try red; auto using star_refl. discriminate.
+
+  - (* Case "BEq". *)
+  eapply (comp_bop_correct bop_eq); auto.
+
+  - (* Case "BLe". *)
+  eapply (comp_bop_correct bop_le); auto.
+
+  - (* Case "BNot". *)
+  simpl. evar (SPEC : mem -> nat). replace (fun (m:mem) => b2n _) with SPEC.
+  subst SPEC. apply (comp_bop_correct bop_eq); eauto.
+  unfold comp_correct; intros. inversion H; subst; clear H.
+  instantiate (1:=fun m => 0).
+  exists st; repeat split; try red; auto using star_refl. discriminate.
+  unfold SPEC. apply functional_extensionality. intro.
+  destruct (beval b x); auto.
+
+  - (* Case "BAnd". *)
+  simpl. evar (SPEC : mem -> nat). replace (fun (m:mem) => b2n _) with SPEC.
+  subst SPEC. apply (comp_bop_correct bop_and); eauto.
+  subst SPEC. apply functional_extensionality. intro. 
+  simpl. destruct (beval b1 x), (beval b2 x); auto.
+Qed.
+
+
+(**
+  - First we define some helper definitions for compiling assignments and 
+    conditionals.
+    - To simplify the simulation: each store is compiled to its own basic block.
+  - Then we define the command compilation context as a state monad.
+    - Generate fresh uids (like the [ectmon])
+    - Generate fresh block labels 
+    - Add instructions to the (partial) CFG
+  - Then we define the translation of commands (recursively).
+*)
+
+
+Lemma comp_store_correct : 
+  forall g a v le lr cs st,
+  insns_at_pc g (block_entry le) (strun (comp_store a v lr) cs) ->
+  st_pc st = (block_entry le) ->
+  exists st',
+    plus (step g) st st' /\
+    st_pc st' = (block_entry lr) /\
+    st_mem st' = (Memory.update (st_mem st) v (aeval a (st_mem st))).
+Proof.
+  intros.
+  unfold strun, comp_store in H. simpl in H.
+  match type of H with context[let (_,_) := ?x in _] => destruct x eqn:Hc end.
+  destruct p as [x is].
+  simpl in H. symmetry in Hc.
+  
+  rewrite <- H0 in H.
+  eelim (comp_aexp_correct a); eauto.
+  intros st' H'. decompose [and] H'; clear H'.
+  rename st' into st''. set (st' := st'') in *. destruct st''.
+
+  eexists.
+  split. eapply plus_star_trans'. eauto. 
+  eapply plus_left. eapply step_store. apply H3. eauto.
+  eapply star_step. eapply step_tmn. inversion H3. apply H9.
+  reflexivity.
+  eapply star_refl.
+  simpl. split; auto.
+  rewrite <- H1. reflexivity.
+Qed.
+
+
+Lemma comp_cond_correct :
+  forall g cs b le l1 l2 st,
+  insns_at_pc g (block_entry le) (strun (comp_cond b l1 l2) cs) ->
+  st_pc st = (block_entry le) ->
+  exists st',
+    plus (step g) st st' /\
+    st_pc st' = block_entry (if beval b (st_mem st) then l1 else l2) /\
+    st_mem st = st_mem st'.
+Proof.
+  intros.
+  unfold strun, comp_cond in H. simpl in H.
+  match type of H with context[let (_,_) := ?x in _] => destruct x eqn:Hc end.
+  destruct p as [x is].
+  simpl in H. symmetry in Hc.
+
+  rewrite <- H0 in H.
+  eelim (comp_bexp_correct b); eauto.
+  intros st' H'. decompose [and] H'; clear H'.
+  rename st' into st''. set (st' := st'') in *. destruct st''.
+
+  eexists.
+  split. eapply plus_star_trans'. eauto. 
+  eapply plus_one. eapply step_tmn. 
+  apply H3. simpl in *. rewrite H8. reflexivity.
+  simpl. split; auto.
+  destruct (beval b (st_mem st)); simpl; auto.
+Qed.
+  
+
+(* ================================================================= *)
+(* ** Compiling Commands *)
+
+(** State:
+    - list of used block labels
+    - list of used uids
+    - current cfg *)
+
+Definition cstate := (list lbl * list uid * list ListCFG.block)%type.
+Notation ctmon := (ST cstate).
+
+Definition fresh_lbl : ctmon lbl :=
+  fun cs =>
+  let '(ls, is, bs) := cs in
+  let l := Lbl.fresh ls in 
+  (l::ls, is, ListCFG.update bs l [], l).
+
+Definition raise_ectmon {T} (ec:ectmon T) : ctmon T :=
+  fun cs =>
+  let '(ls, is, cfg) := cs in
+  let (is', r) := ec is in
+  (ls, is', cfg, r).
+
+Definition add_insns (l:lbl) (b:list insn) : ctmon unit :=
+  fun cs =>
+  let '(ls, is, cfg) := cs in
+  (ls, is, ListCFG.update cfg l b, tt).
+
+Open Scope imp_scope.
+
+(* ################################################################# *)
+(** * Correctness? *)
+
+(** - Vminus is deterministic
+    - Suffices to show a forward simulation. *)
+
+(* ================================================================= *)
+(** ** Simulation relation. *)
+
+(** Relate Imp commands to sequences of basic blocks in the cfg. *)
+
+Inductive match_config : Imp.com -> (ListCFG.t * lbl * lbl) -> Prop :=
+  | MC_Skip : forall bs l,
+      match_config SKIP (bs, l, l)
+  | MC_Ass : forall g l l' uid a cs,
+      insns_at_pc g (block_entry l) (strun (comp_store a uid l') cs) ->
+      match_config (CAss uid a) (g, l, l')
+  | MC_Seq : forall g l1 l2 l3 c1 c2,
+      match_config c1 (g, l1, l2) ->
+      match_config c2 (g, l2, l3) ->
+      match_config (CSeq c1 c2) (g, l1, l3)
+  | MC_If : forall g le lr l1 l2 b c1 c2 cs,
+      match_config c1 (g, l1, lr) ->
+      match_config c2 (g, l2, lr) ->
+      insns_at_pc g (block_entry le) (strun (comp_cond b l1 l2) cs) ->
+      match_config (CIf b c1 c2) (g, le, lr)
+  | MC_While : forall g le lb lr b c cs,
+      match_config c (g, lb, le) ->
+      insns_at_pc g (block_entry le) (strun (comp_cond b lb lr) cs) ->
+      match_config (CWhile b c) (g, le, lr).
+
+Inductive match_states (g:ListCFG.t) (r:lbl)
+  : (com * Imp.state) -> state -> Prop :=
+  match_states_intro : forall c mem st l,
+    match_config c (g, l, r) ->
+    st_pc st = block_entry l ->
+    st_mem st = mem ->
+    match_states g r (c, mem) st.
+
+
+Require Import Program.Equality.
+
+(* ================================================================= *)
+(** ** Translation simulation: First try. *)
+
+Lemma simulation_step' :
+  forall g c c' mem mem' st r,
+  Imp.step (c, mem) (c', mem') ->
+  match_states g r (c, mem) st ->
+  exists st',
+    star (step g) st st' /\
+    match_states g r (c', mem') st'.
+Proof.
+  intros. generalize dependent st. revert r.
+  
+  dependent induction H; intros;
+  inversion H0 as [? ? ? ? H']; inversion H'; subst.
+
+  - (* Case "S_Ass". *)
+  eapply comp_store_correct in H6 as [st' [? [? ?]]]; eauto.
+  eexists. split. apply plus_star. apply H1. econstructor; eauto. apply MC_Skip. 
+
+  - (* Case "S_Seq". *)
+    specialize (IHstep c1 c1' (st_mem st) mem').
+    pose (K:=IHstep ltac:(auto) ltac:(auto)); clearbody K; clear IHstep.
+    specialize (K l2 st).
+    lapply K.
+    intros [st' [? ?]].
+    exists st'. split; auto.
+    inversion H3. 
+    econstructor; eauto. econstructor; eauto.
+    econstructor; eauto.  
+
+  - (* Case "S_SeqSkip". *)
+  exists st. split. apply star_refl.
+  inversion H'; subst. inversion H4; subst.
+  econstructor; eauto.
+
+  - (* Case "S_IfTrue". *)
+  eapply comp_cond_correct in H14 as [st' [? [? ?]]].
+  exists st'. split. apply plus_star; eauto. econstructor. 
+  eauto. rewrite H in H3. auto. symmetry; auto. auto.
+
+  - (* Case "S_IfFalse". *)
+  eapply comp_cond_correct in H14 as [st' [? [? ?]]].
+  exists st'. split. apply plus_star; eauto. econstructor. 
+  eauto. rewrite H in H3. auto. symmetry; auto. auto.
+
+  - (* Case "S_While". *)
+  exists st. split. apply star_refl. 
+  econstructor; eauto. eapply MC_If; eauto.
+  econstructor; eauto. apply MC_Skip; eauto.
+Qed.
+
+(* ################################################################# *)
+(** * Stuttering *)
+
+(** The proof above goes through, but does not ensure that if the
+    source program diverges the compiled program does not go wrong! 
+
+    To fix it, we need to ensure that there is no "infinite stuttering"
+    in which the source program takes an infinite number of steps while 
+    the target terminates (or gets stuck).
+*)
+
+(* ================================================================= *)
+(** ** Eliminating Stuttering *)
+
+(** First, define an appropriate measure. *)
+
+Fixpoint num_skips (c:com) : nat :=
+  match c with
+    | (c1 ;; c2) => num_skips c1 + num_skips c2
+    | SKIP => 2
+    | _ => 0
+  end.
+
+Fixpoint while_head (c:com) : nat :=
+  match c with
+    | (c1 ;; _) => while_head c1
+    | WHILE _ DO _ END => 1
+    | _ => 0
+  end.
+
+Definition com_size (c:com) : nat := num_skips c + while_head c.
+
+(* ================================================================= *)
+(** ** Lemmas about the measure. *)
+
+Require Import Omega.
+
+Lemma while_head_bound : forall c, while_head c < 2.
+Proof. induction c; simpl; omega. Qed.
+
+Lemma com_size_seq : forall c1 c1' c2,
+  com_size c1' < com_size c1 ->
+  com_size (c1';; c2) < com_size (c1;; c2).
+Proof.
+  unfold com_size; destruct c1, c1'; 
+  try solve [simpl; intros; omega].
+Qed.
+
+Lemma com_size_seqskip : forall c,
+  com_size c < com_size (SKIP;; c).
+Proof.
+  unfold com_size; destruct c;
+  try solve [simpl; try match goal with
+                        | |- context[while_head ?X] => 
+                             pose proof (while_head_bound X)
+                        end; intros; omega].
+Qed.
+
+
+(* lift to states *)
+Definition imp_size (st:com * mem) : nat := 
+  let (c, _) := st in com_size c.
+
+
+
+Local Hint Constructors match_config.
+Hint Resolve com_size_seqskip com_size_seq.
+
+(* ================================================================= *)
+(** ** Final simulation relation. *)
+
+Lemma transl_sim_step_final :
+  forall g r imp_st imp_st' vmn_st,
+  Imp.step imp_st imp_st' ->
+  match_states g r imp_st vmn_st ->
+  exists vmn_st',
+    (plus (step g) vmn_st vmn_st' \/
+     star (step g) vmn_st vmn_st' /\ imp_size imp_st' < imp_size imp_st) /\
+    match_states g r imp_st' vmn_st'.
+Proof.
+  intros. generalize dependent vmn_st. revert r.
+  
+  dependent induction H; intros r vmn_st Hst;
+  inversion Hst as [? ? ? ? Hcfg]; inversion Hcfg; subst.
+
+  - (* Case "S_Ass". *)
+  eapply comp_store_correct in H6 as [st' [? [? ?]]]; eauto.
+  eexists. split; eauto. econstructor; eauto.
+  
+  - (* Case "S_Seq". *)
+  specialize (IHstep l2 vmn_st).
+  lapply IHstep. intros [vmn_st' [? ?]]. exists vmn_st'. split. 
+  simpl in *; intuition. inversion H2; subst. 
+  econstructor; eauto. econstructor; eauto.
+
+  - (* Case "S_SeqSkip". *)
+  exists vmn_st. split. right. 
+  split. apply star_refl. unfold imp_size. 
+  simpl; intuition. inversion H7; subst. econstructor; eauto.
+
+  - (* Case "S_IfTrue". *)
+  eapply comp_cond_correct in H13 as [st' [? [? ?]]]; eauto.
+  exists st'. split; eauto. econstructor; eauto. 
+  rewrite H in H2; auto. 
+
+  - (* Case "S_IfFalse". *)
+  eapply comp_cond_correct in H13 as [st' [? [? ?]]]; eauto.
+  exists st'. split; eauto. econstructor; eauto.  
+  rewrite H in H2; auto. 
+
+  - (* Case "S_While". *)
+  exists vmn_st. split. right; intuition. apply star_refl. 
+  econstructor; eauto. 
+Qed.
+
+(** Is this enough? *)
+
+(* ================================================================= *)
+(** ** Relating initial states *)
+
+(** We still must relate the initial states! *)
+
+(** First, some helpers: *)
+
+Require Import Vminus.LtacDebug.
+
+Lemma comp_store_not_nil : forall a v l cs,
+  strun (comp_store a v l) cs <> [].
+Proof.
+  intros. unfold strun.
+  remember (comp_store _ _ _ _) as ma.
+  unfold comp_store in Heqma. simpl in Heqma.
+  match type of Heqma with context[let (_,_) := ?x in _] => destruct x eqn:Hc end.
+  destruct p as [v' is].
+  subst ma; simpl. intro.
+  eapply app_cons_not_nil; eauto.
+Qed.
+
+Lemma comp_cond_not_nil : forall b v l cs,
+  strun (comp_cond b v l) cs <> [].
+Proof.
+  intros. unfold strun.
+  remember (comp_cond _ _ _ _) as ma.
+  unfold comp_cond in Heqma. simpl in Heqma.
+  match type of Heqma with context[let (_,_) := ?x in _] => destruct x eqn:Hc end.
+  destruct p as [v' is].
+  subst ma; simpl. intro.
+  eapply app_cons_not_nil; eauto.
+Qed.
+
+(* ================================================================= *)
+(** ** Compilation invariant *)
+
+(** Compilation only "extends" the compilation state:
+    - Uids and labels change only monotonically.
+    - Compilation never removes code.
+  *) 
+
+Inductive cstate_incr : cstate -> cstate -> Prop :=
+  cstate_incr_intro : forall ls ls' ids ids' g g',
+    (forall l, In l ls -> In l ls') ->
+    (forall l is, In l ls -> is <> nil ->
+      ListCFG.lookup g  l = Some is -> ListCFG.lookup g' l = Some is) ->
+    cstate_incr (ls, ids, g) (ls', ids', g').
+
+Instance cstate_incr_trans : Transitive cstate_incr.
+Proof.
+  red. inversion 1. inversion 1. constructor; intuition.
+Qed.
+
+Inductive cstate_incr_strong : cstate -> cstate -> Prop :=
+  cstate_incr_strong_intro : forall ls ls' ids ids' g g',
+    (forall l, In l ls -> In l ls') ->
+    (forall l, In l ls -> ListCFG.lookup g l = ListCFG.lookup g' l) ->
+    cstate_incr_strong (ls, ids, g) (ls', ids', g').
+
+Instance cstate_incr_strong_trans : Transitive cstate_incr_strong.
+Proof.
+  red. inversion 1. inversion 1. subst. constructor. 
+  auto. intros. transitivity (ListCFG.lookup g' l); eauto.
+Qed.
+
+
+Instance cstate_incr_strong_refl : Reflexive cstate_incr_strong.
+Proof.
+  red. intro cs. destruct cs as [[? ?] ?]. constructor; auto.
+Qed.
+
+
+Lemma add_insns_incr : forall l is g ls ids cs',
+  ListCFG.lookup g l = Some [] ->
+  add_insns l is (ls, ids, g) = (cs', tt) ->
+  cstate_incr (ls, ids, g) cs'.
+Proof.
+  destruct cs' as [[? ?] ?]. intros.
+  constructor. inversion H0; intuition.
+  intros. inversion H0; subst. rewrite ListCFG.update_neq. auto.
+  contradict H2. subst l. rewrite H3 in H. injection H; auto.
+Qed.
+
+
+Lemma ectmon_incr_strong : 
+  forall (A:Type) (m:ectmon A) (r:A) cs cs' ,
+  raise_ectmon m cs = (cs', r) ->
+  cstate_incr_strong cs cs'.
+Proof.
+  destruct cs as [[? ?] ?], cs' as [[? ?] ?].
+  inversion 1.
+  destruct (m l0). inversion H1; subst; clear H1.
+  constructor; auto; intros. 
+Qed.
+
+
+Lemma fresh_add_incr_strong :
+  forall l is cs1 cs2 cs3 cs4,
+  fresh_lbl cs1 = (cs2, l) ->
+  cstate_incr_strong cs2 cs3 ->
+  add_insns l is cs3 = (cs4, tt) ->
+  cstate_incr_strong cs1 cs4.
+Proof.
+  intros until cs4. intros Hfresh Hincr Hadd.
+  destruct cs1 as [[? ?] ?], cs2 as [[? ?] ?],
+           cs3 as [[? ?] ?], cs4 as [[? ?] ?].
+  inversion Hadd; inversion Hfresh; inversion Hincr; subst.
+
+  constructor; intros. apply H8. right; auto.
+  assert (Lbl.fresh l0 <> l).
+    contradict H. rewrite <- H. apply Lbl.fresh_not_in.
+  rewrite ListCFG.update_neq; auto. rewrite <- H13.
+  rewrite ListCFG.update_neq; auto. right; auto.
+Qed.
+
+Ltac bind_step H :=
+  match type of H with
+  | context[let (_,_) := ?b in _] => destruct b as [?x ?y] eqn:?Hb
+  end.
+
+
+Ltac compile :=
+  repeat
+    match goal with
+    | [ x : Compiler.cstate |- _] => destruct x as [[?lbls ?ids] ?bs] 
+(*    | [ H : context[Compiler.add_insns _ _ _] |- _ ] => simpl in H *)
+    | [ H : context[let (_,_) := ?x in _] |- _] => destruct x as [?l ?r] eqn:?Heq
+    | [ H : (_, _) = (_, _) |- _] => inversion H; subst; clear H
+    | [ H : () |- _ ] => destruct H
+    end.
+
+Lemma comp_com_incr_strong: forall c cst cst' e r,
+  comp_com c r cst = (cst', e) -> cstate_incr_strong cst cst'.
+Proof.
+  induction c; intros cst cst' e r Htr; simpl in Htr; compile.
+
+  - (* Case "CSkip".*)
+    reflexivity. 
+
+  - (* Case "CAss". *) 
+  eapply fresh_add_incr_strong; eauto.
+  eapply ectmon_incr_strong; eauto. 
+
+  - (* Case "CSeq". *)
+  eapply transitivity.
+  eapply IHc2; eauto.  eapply IHc1; eauto.
+
+  -  (* Case "CIf". *)
+  eapply transitivity. eapply IHc1; eauto.
+  eapply transitivity. eapply IHc2; eauto.
+  eapply fresh_add_incr_strong; eauto. 
+  eapply ectmon_incr_strong; eauto.
+
+  - (* Case "CWhile". *)
+  eapply fresh_add_incr_strong.
+  eauto. eapply transitivity. eapply IHc; eauto.
+  eapply ectmon_incr_strong; eauto. eauto.
+Qed.
+  
+
+Lemma cstate_incr_weaken : forall cst cst',
+  cstate_incr_strong cst cst' ->
+  cstate_incr cst cst'.
+Proof.
+  inversion 1. constructor. auto. intros. rewrite <- H1; auto.
+Qed.
+
+Lemma comp_com_incr: forall c cst cst' e r,
+  comp_com c r cst = (cst', e) -> cstate_incr cst cst'.
+Proof.
+  intros. apply cstate_incr_weaken.
+  eapply comp_com_incr_strong; eauto.
+Qed.
+
+(* ================================================================= *)
+(** ** Relating Initial Compilation *)
+
+(** The key lemma is: *)
+
+Lemma match_init : forall c le lr csti cst x g' e,
+  comp_com c lr csti = (cst, le) ->
+  cstate_incr cst (x, g') ->
+  match_config c (e, g', le, lr).
+Proof.
+  induction c; intros le lr csti cst x g' e Hcomp Hincr; simpl in Hcomp; compile.
+  
+  - (* Case "CSkip". *)
+  apply MC_Skip.
+
+  - (* Case "CAss". *)
+    simpl in Heq. inversion Heq; subst; clear Heq.
+    simpl in Heq0.
+    destruct (comp_store a i lr ids1) eqn:Hc'.
+    inversion Heq0; subst; clear Heq0.
+    simpl in Heq1.
+    inversion Heq1; subst; clear Heq1.
+
+    eapply MC_Ass, cfg_insns_at.
+    inversion Hincr. subst. 
+    apply H5. left; auto.
+    apply comp_store_not_nil. rewrite ListCFG.update_eq; auto. 
+    f_equal. rewrite surjective_pairing in Hc' at 1. 
+    inversion Hc'. reflexivity.
+
+  - (* Case "CSeq". *)
+    eapply MC_Seq. eapply IHc1; eauto. eapply IHc2; eauto.
+    eapply transitivity; eauto. eapply comp_com_incr; eauto.
+
+  - (* Case "CIf". *)
+    eapply MC_If.
+
+    + eapply IHc1; eauto.
+      eapply transitivity. eapply comp_com_incr; eauto.
+      eapply transitivity; eauto. eapply cstate_incr_weaken. 
+      eapply fresh_add_incr_strong; eauto.
+      eapply ectmon_incr_strong; eauto.
+
+    + eapply IHc2; eauto.
+      eapply transitivity; eauto. eapply cstate_incr_weaken.
+      eapply fresh_add_incr_strong; eauto.
+      eapply ectmon_incr_strong; eauto.
+
+    + inversion Heq1. subst. clear Heq1.
+      simpl in Heq2.
+      compile.
+      inversion Heq3. subst. clear Heq3.
+      eapply cfg_insns_at.
+      inversion Hincr. subst.
+      apply H5. left; auto.
+      apply comp_cond_not_nil.
+      rewrite ListCFG.update_eq; auto. 
+      f_equal.
+      rewrite surjective_pairing in Heq1 at 1. 
+      inversion Heq1. reflexivity.
+      
+  - (* Case "CWhile". *)
+    eapply MC_While with (cs:=ids2).
+
+    + simpl in Heq. inversion Heq; subst. clear Heq.
+    
+      eapply IHc. eauto.
+      apply comp_com_incr_strong in Heq0.
+      apply ectmon_incr_strong in Heq1.
+      eapply transitivity; eauto.
+      eapply transitivity; eauto.
+      eapply cstate_incr_weaken; eauto.
+      apply add_insns_incr in Heq2; eauto.
+
+      inversion Heq1. subst. rewrite <- H6.
+      inversion Heq0. subst. rewrite <- H8. 
+      rewrite ListCFG.update_eq; auto.
+      left. auto.
+      inversion Heq0. subst. apply H2. left. auto.
+
+    + inversion Heq.  subst.
+
+      apply cfg_insns_at.
+      inversion Hincr. subst. 
+      apply H5.
+
+      apply comp_com_incr_strong in Heq0.
+      apply ectmon_incr_strong in Heq1.      
+      inversion Heq0. subst.
+      inversion Heq2. subst.
+      inversion Heq1. subst.
+      apply H3. apply H2. left. reflexivity.
+      
+      apply comp_cond_not_nil.
+      
+      inversion Heq2. subst. rewrite ListCFG.update_eq; auto.
+      f_equal. rewrite surjective_pairing in Heq1 at 1.
+      inversion Heq1. subst. unfold strun.
+      destruct (comp_cond b r0 lr ids2). reflexivity.
+Qed.
+
+
+(* adapted from Leroy, OPLSS '12 Compil.v *)
+(* Generic simulation proof. *)
+
+Section SIMULATION_DIAGRAM.
+
+Variable state1: Type.	                          (* source states *)
+Variable step1: state1 -> state1 -> Prop.         (* source step relation *)
+
+Variable state2: Type.	                          (* target states *)
+Variable step2: state2 -> state2 -> Prop.         (* target step relation *)
+
+Variable match_states: state1 -> state2 -> Prop.  (* the invariant *)
+
+Variable measure: state1 -> nat.                  (* for stuttering *)
+
+Hypothesis simulation:
+  forall S1 S1' S2,
+  step1 S1 S1' -> match_states S1 S2 ->
+  exists S2',
+    (plus step2 S2 S2' \/ 
+     star step2 S2 S2' /\ measure S1' < measure S1) /\
+    match_states S1' S2'.
+
+Lemma simulation_star:
+  forall S1 S1', star step1 S1 S1' ->
+  forall S2, match_states S1 S2 ->
+  exists S2', star step2 S2 S2' /\ match_states S1' S2'.
+Proof.
+  induction 1; intros.
+
+  - (* Case "zero transition". *)
+  exists S2; split. apply star_refl. auto.
+
+  - (* Case "one or more transitions". *)
+  destruct (simulation _ _ _ H H1) as [S2' [P Q]].
+  destruct (IHstar _ Q) as [S2'' [U V]].
+  exists S2''; split. 
+  eapply star_trans; eauto. destruct P. 
+  apply plus_star; auto. destruct H2; auto.
+  auto.
+Qed.
+
+Lemma simulation_infseq_productive:
+  forall N S1 S2,
+  measure S1 < N ->
+  infseq step1 S1 ->
+  match_states S1 S2 ->
+  exists S1', exists S2',
+      plus step2 S2 S2'
+   /\ infseq step1 S1'
+   /\ match_states S1' S2'.
+Proof.
+  induction N; intros. 
+  - (* Case "N = 0". *)
+  omega. 
+  - (* Case "N > 0". *)
+  inversion H0; clear H0; subst.
+  destruct (simulation _ _ _ H2 H1) as [S2' [P Q]].
+  destruct P.
+  + (* SCase "one or several transitions". *)
+  exists b; exists S2'; auto.
+  + (* SCase "zero, one or several transitions". *)
+  destruct H0. inversion H0; clear H0; subst.
+    * (* SSCase "zero transitions". *)
+    eapply IHN; eauto. omega.
+    * (* SSCase "one or several transitions". *)
+    exists b; exists S2'; split. eapply plus_left; eauto. auto.
+Qed.
+
+Lemma simulation_infseq:
+  forall S1 S2,
+  infseq step1 S1 ->
+  match_states S1 S2 ->
+  infseq step2 S2.
+Proof.
+  intros. 
+  apply infseq_coinduction_principle_2 with
+    (X := fun S2 => exists S1, infseq step1 S1 /\ match_states S1 S2).
+  intros. destruct H1 as [S [A B]]. 
+  destruct (simulation_infseq_productive (measure S + 1) S a) 
+  as [S1' [S2' [P [Q R]]]].
+  omega. auto. auto.
+  exists S2'; split. auto. exists S1'; auto. 
+  exists S1; auto.
+Qed.
+
+End SIMULATION_DIAGRAM.
+
+
+Definition vminus_terminates (g:ListCFG.t) (m m':mem) : Prop :=
+  exists x st',
+    insns_at_pc g st'.(st_pc) [(x, cmd_tmn tmn_ret)] /\
+    st'.(st_mem) = m' /\
+    star (step g) (init_state g m) st'.
+  
+Definition vminus_diverges (g:ListCFG.t) (m:mem) : Prop :=
+  infseq (step g) (init_state g m).
+
+Definition imp_terminates (c: com) (m m':mem) : Prop :=
+  star Imp.step (c, m) (SKIP, m').
+
+Definition imp_diverges (c: com) (mem: mem) : Prop :=
+  infseq Imp.step (c, mem).
+
+Lemma match_config_ret : forall g le lr c,
+  (g, le, lr) = compile c ->
+  exists x, insns_at_pc g (block_entry lr) [(x, cmd_tmn tmn_ret)].
+Proof.
+  intros. unfold compile, comp_prog in H. simpl in H. compile.
+  
+  eexists. eapply cfg_insns_at. apply comp_com_incr_strong in Heq1.
+  inversion Heq1; subst. rewrite <- H6. rewrite ListCFG.update_eq; auto.
+  left. reflexivity.
+Qed.
+
+Lemma match_config_initial : forall g le lr c m,
+  (g, le, lr) = compile c ->
+  match_states g lr (c, m) (init_state g m).
+Proof.
+  intros. unfold compile, comp_prog in H. simpl in H. compile.
+  econstructor; simpl; eauto.
+
+  eapply match_init. eauto. eapply cstate_incr_weaken. 
+  eapply cstate_incr_strong_refl.
+Qed.
+
+Theorem compile_program_correct_terminating:
+  forall c m m' g le lr,
+  (g, le, lr) = compile c ->
+  imp_terminates c m m' ->
+  vminus_terminates g m m'.
+Proof.
+  intros. unfold imp_terminates in H.
+  assert (exists machconf2, 
+           star (step g) (init_state g m) machconf2
+           /\ match_states g lr (SKIP, m') machconf2).
+  eapply simulation_star; eauto. eapply transl_sim_step_final. 
+  eapply match_config_initial; eauto.
+  destruct H1 as [machconf2 [STAR MS]]. 
+  inversion MS; subst.
+  eelim match_config_ret. intros.
+  red. exists x, machconf2. split. rewrite H4. eauto. eauto. 
+  inversion H3; subst. eauto.
+Qed.
+
+Theorem compile_program_correct_diverging:
+  forall c m g le lr,
+  (g, le, lr) = compile c ->
+  imp_diverges c m ->
+  vminus_diverges g m.
+Proof.
+  intros; red; intros. 
+  eapply simulation_infseq with (match_states := match_states g lr); eauto.
+  eapply transl_sim_step_final. eapply match_config_initial; eauto.
+Qed.
