vminus/CompilerTest.v
@@ -1,0 +1,820 @@
+Require Import List.
+Import ListNotations.
+Require Import String.
+Require Import Arith.
+
+Require Import QuickChick.QuickChick.
+Import QcDefaultNotation. Open Scope qc_scope.
+
+Require Import Vminus.Classes.
+Require Import Vminus.Vminus.
+Require Import Vminus.Atom.
+Require Import Vminus.CFG.
+Require Import Vminus.ListCFG.
+Require Import Vminus.Imp.
+Require Import Vminus.Compiler.
+Require Import Vminus.VminusOpSem. (* More refactoring work to do *)
+Import V.Opsem.
+
+(* Exercise imports *)
+Require Import Vminus.AtomGen.
+Require Import Vminus.ImpGen.
+Require Import Vminus.OpSemGen.
+Require Import Vminus.Stmon.
+
+(** ** QuickChick and Vellvm **************************************************)
+(** One may expect a compiler for a language as simple as IMP to be relatively 
+    straightforward, and a proof of its correctness to be correspondingly
+    so. However, LLVM is a full-featured IR, and a faithful formalization 
+    is necessarily complex and large. When the compiler is under development, 
+    even stating the correctness of the compiler can be difficult, much 
+    less prove it.
+
+    But if we have interpreters for both the source and target, testing the 
+    compiler is a much simpler affair. Moreover, the simplicity of the source 
+    language, i.e. Imp. means that it is really easy to test! *)
+
+(** This lecture shows how QuickChick can be used to test the compiler. For
+    simplicity, the target language is the simplified SSA language Vminus, and
+    we use a variant of Imp whose names are just memory addresses which can be 
+    interpreted in the memory of Vminus states. Imp states and Vminus memory
+    are hence essentially the same, and this makes it easy to state correct 
+    compilation: after running the source program and its compilation, 
+    every Imp variable/address is mapped to the same nat by both the Imp state 
+    and Vminus memory. 
+
+    A Vminus state consists of a memory (mapping addresses to nat), a program 
+    counter, an environment mapping locals to nat, a "previous" program 
+    counter, and a "previous" environment. The latter two are needed for
+    executing phi nodes. A configuration consists of a Vminus state and a CFG,
+    which "holds" Vminus instructions organized in basic blocks.
+*)
+
+(** Here's a look at what we mean. 
+
+Theorem compile_program_correct_terminating:
+  forall c m m' g le lr,
+  (g, le, lr) = compile c ->
+  imp_terminates c m m' ->
+  vminus_terminates g m m'.
+
+  This is one of the top-level correctness theorems for the compiler: for any 
+  initial memory m, if the source program c terminates with memory (Imp state) 
+  m', running the compilation result g (a control flow graph holding the 
+  instructions) on the same initial memory m also results in termination, and
+  with its final (Vminus) memory also being m. This is where the coincidence of 
+  Imp states and Vminus memory comes into play.
+  
+  Terminating Imp programs are those that are evaluated to just SKIP, as the
+  following definition shows. 
+
+  Definition imp_terminates (c: com) (m m':mem) : Prop :=
+    star Imp.step (c, m) (SKIP, m').
+
+  For Vminus programs on the other hand, running them on an initial memory m 
+  leads to termination with memory m' if execution reaches some uid x 
+  associated with a return terminator.
+
+  Definition vminus_terminates (g:ListCFG.t) (m m':mem) : Prop :=
+    exists x st',
+      insns_at_pc g st'.(st_pc) [(x, cmd_tmn tmn_ret)] /\
+      st'.(st_mem) = m' /\
+      star (step g) (init_state g m) st'.
+
+  The variables x and st' here are determined by "running"/evaluation, as 
+  indicated by "star (step g) (init_state g m) st'". So checking for their 
+  existence is really verifying that an evaluation function reaches st' 
+  satisfying the constraints. 
+ *)
+
+(** Let us try to write a Checker for the theorem. Looking at the universals, 
+    it would appear that we need generators for Imp commands (c), Imp 
+    states/memories (m, m'), control flow graphs (g) and labels (le, lr).
+    However, note that g, le, and lr are computed by "compile c", so we 
+    don't actually need generators for them. Moreover, we do not want just any 
+    c and m', but only terminating Imp programs, and m' is obtained by running
+    an Imp evaluator on m. Hence for generation, we only need:
+    - A generator for mem. 
+    - A generator for Imp programs that are guaranteed to terminate. 
+    And for checking, we would need:
+    - An evaluator for Imp that reaches termination, i.e. SKIP.
+    - An evaluator for Vminus that reaches termination, i.e. a return 
+      terminator. 
+    - We also need to check that the final state st' that the Vminus evaluator 
+      reaches has the desired memory.
+*)
+
+(** Let us first define an evaluator for Vminus. The evaluator stops when 
+    a return terminator is reached. *)
+
+Fixpoint vminus_eval (g: ListCFG.t) (s : state) (fuel: nat) : err state :=
+  (* FILL IN HERE *)
+  match fuel with
+  | 0 => inl "out of fuel"
+  | S n' =>
+    match (ListCFG.fetch g (st_pc s)) with
+    | Some instr =>
+      if eq_dec_cmd (snd instr) (cmd_tmn tmn_ret) then inr s
+      else
+        match (eval_step g s) with
+        | inr s' => vminus_eval g s' n'
+        | inl err => inl err
+        end
+    | None => inl "no instr to fetch"
+    end
+  end.
+
+(** It is likely that QuickChick will generate large enough Imp programs such 
+    that vminus_eval can run out of fuel. (Think of large aexp expressions.)
+
+    Exercise: Write an instance of GenSized for aexp and bexp such that 
+    any size above a certain number, say 5, is rounded down to that. The 
+    GenSized instance for bexp should make use of that for aexp. 
+ *)
+
+Derive Arbitrary for aexp.
+
+Definition round_down_to (n: nat) (k: nat) :=
+  if (lt_dec n k) then n else k.
+
+Instance gen_small_aexp: GenSized aexp :=
+  (* FILL IN HERE *)
+  {| arbitrarySized n := @arbitrarySized aexp _ (round_down_to 5 n)
+  |}.
+
+Instance gen_small_bexp: GenSized bexp :=
+  (* FILL IN HERE *)
+  {| arbitrarySized n :=
+       let fix gen_bexp_func n :=
+           match n with
+           | 0 => elems [BTrue ; BFalse]
+           | S n' =>
+             let beq_gen := liftGen2 BEq
+                                     (arbitrarySized n)
+                                     (arbitrarySized n) in
+             let ble_gen := liftGen2 BLe
+                                     (arbitrarySized n)
+                                     (arbitrarySized n) in
+           let bnot_gen := liftGen BNot (gen_bexp_func n') in
+           let band_gen := liftGen2 BAnd (gen_bexp_func n') (gen_bexp_func n')
+           in
+           oneOf [ beq_gen ; ble_gen ; bnot_gen ; band_gen ]
+           end in
+       gen_bexp_func (round_down_to 5 n)
+  |}.
+
+(** For com, recall that the lemma applies only to terminating ones. Hence, 
+    write two sized generators for com: 
+    - one that generates only assignment statements and SKIPs, such that the 
+      latter are generated with low probability.
+    - one that generates IF-THEN-ELSE, assignments and SKIPs, but no loops.
+ *)
+
+Fixpoint gen_seq_com (n : nat) : G com :=
+  (* FILL IN HERE *)
+  match n with 
+  | 0 => freq [(4, liftGen2 CAss arbitrary arbitrary); (1, returnGen SKIP)]
+  | S n' =>
+    let gen := gen_seq_com n' in
+    liftGen2 CSeq gen gen
+  end. 
+
+Fixpoint gen_if_com (n: nat) : G com :=
+  (* FILL IN HERE *)
+  match n with
+  | 0 => freq [(1, returnGen CSkip) ;
+                (4, liftGen2 CAss arbitrary arbitrary)]
+  | S n' =>
+    let gen := gen_if_com n' in
+    oneOf [liftGen3 CIf arbitrary gen gen; liftGen2 CSeq gen gen]
+  end.
+
+(** For your convenience, the Shows and Shrinks for aexp, bexp and com have 
+    been defined. *)
+
+(** The last thing we need a generator for is mem. One could generate this by 
+    first generating a subset of its domain, i.e. Atom.t, and then generating 
+    the image for this subset; the rest would be kept as some initial value. 
+*)
+
+(** Write a function that outputs a generator for mem, given a list of 
+    atoms. 
+*)
+
+Definition gen_mem_from_atom_list
+           (atom_list : list Atom.t) : G mem :=
+  (* FILL IN HERE *)
+  bindGen (vectorOf (List.length atom_list) arbitrary) (fun nat_list => 
+  returnGen (fun (a : Atom.t) =>
+               match (index_of_atom_in_list a atom_list) with
+               | None => 0
+               | Some i =>
+                 List.nth i nat_list 0
+               end)).
+
+(** Now write a generator for Atom.t. You may find the function get_fresh_atoms
+    useful: it takes in (n: nat) and a list of atoms, and outputs a list of n
+    atoms that are distinct from the input. 
+*)
+
+Check get_fresh_atoms 6 [].
+
+Instance gen_domain : Gen Atom.t :=
+  (* FILL IN HERE *)  
+  {| arbitrary :=
+       let atom_store := get_fresh_atoms 100 [] in
+       oneof (returnGen (Atom.fresh [])) (List.map returnGen atom_store)
+  |}.
+
+(** It would be convenient to show memory too. *)
+
+Check show_memory.
+
+(** With generation out of the way, we can now return to checking. 
+    The Vminus evaluator defined earlier solves a part of the puzzle, namely
+    the question of how to check the existence of st' and x. However, we also 
+    need to check that st' has the desired memory. Because memories here are 
+    total maps, we can only check for equality of memories for a specified 
+    domain. 
+*)
+
+Fixpoint memory_on_domain_checker
+         (dom: list addr) (mem1 mem2 : V.Opsem.mem) : Checker :=
+  match dom with
+  | [] => checker true
+  | (a :: l) =>
+    if Nat.eqb (mem1 a) (mem2 a) then
+      memory_on_domain_checker l mem1 mem2
+    else
+      whenFail
+        ("memory_equal: memory at " ++ (show a)
+                                    ++ " not equal:"
+                                    ++ " mem1 has " ++ (show (mem1 a))
+                                    ++ "; mem2 has " ++ (show (mem2 a))
+        )%string
+        false
+  end.
+
+(** This lets us assemble the termination checker for Vminus in full. *)
+Definition vminus_termination_checker
+           (g: ListCFG.t) (m m': mem) (dom: list addr) : Checker :=
+  (* FILL IN HERE *)
+  match vminus_eval g (init_state g m) 10000 with
+  | inr final_state =>
+    whenFail "vminus_termination_check: memories not equal"
+             (memory_on_domain_checker dom (st_mem final_state) m')
+  | inl err =>
+    whenFail ("vminus_termination_check: " ++ err) false
+  end.
+
+(** And therefore, the Checker for the lemma in full. *)
+
+Definition compile_program_correct_terminating_checker: Checker :=
+  forAll (gen_seq_com 5) (fun (c : Imp.com) =>
+  forAll arbitrary (fun (dom : list Atom.t) => 
+  forAllShrinkShow (gen_mem_from_atom_list dom)
+                   (fun x => []) (* dummy shrinker *)
+                   (fun m => show_memory m dom) (* show just for the domain *)
+                   (fun m => 
+  let '(g, le, lr) := compile c in
+    match imp_eval c m 100 with
+    | Some s' =>
+      vminus_termination_checker g m s' dom
+    | None => whenFail "compile_program_termination: cannot eval imp to Skip"
+                      false
+    end))).
+
+(** Note the use of forAllShrinkShow here, which lets us choose the specific 
+    Show we want to use; it is needed here because we don't have a Show 
+    instance for total maps like mem. *)
+
+(* ! QuickChick compile_program_correct_terminating_checker. *)
+
+(** For the next part, let us go into the sort of lemmas that would be needed 
+    to prove the top-level correctness theorems like the one above. Here's one.
+
+Lemma comp_aexp_correct : forall (a:aexp),
+    comp_correct (comp_aexp a) (aeval a).
+
+Definition comp_correct (comp : ectmon (val * list insn))
+           (eval : mem -> nat) : Prop :=
+  forall (cs cs': list uid) (g: ListCFG.t) (st: V.Opsem.state)
+    (is k: list insn) (v: val), 
+    (cs', (v, is)) = comp cs ->
+    insns_at_pc g (st_pc st) (is ++ k) ->
+    exists st',
+      st_mem st' = st_mem st /\
+      insns_at_pc g (st_pc st') k /\
+      star (Opsem.step g) st st' /\
+      ids_preserved cs st st' /\
+      good_return cs' v /\
+      ctx_incr cs cs' /\
+      eval_val (st_loc st') v = Some (eval (st_mem st)).
+*)
+
+(** That is, compiling Imp aexp is correct if:
+    - for any compilation run on an initial list of uids, 
+    - wherever we place the compilation result "is" in the CFG, as long
+      as the pc is pointed to it, (insns_at_pc g (st_pc) (is ++ k)),
+    - we can run to the end of compilation (insns_at_pc g (st_pc st') k),
+    - and in this state st', the memory is the same as above; but evaluating 
+      the result of the expression in this state (eval_val (st_loc st') v)
+      is exactly the same as evaluating it according to the Imp state
+      (eval (st_mem st)). 
+    - This last fact may not be obvious from the body of comp_correct. But note 
+      comp_aexp_correct; the evaluation function passed to it is Imp's aeval, 
+      and this is where the coincidence of Imp states and Vminus memory comes 
+      into play.
+    There is a bunch of other things that we need here, so as to prove correct
+    compilation for com. But the above description is the crux.
+*)
+
+(** Looking at comp_correct, it is clear that we need to generate more than 
+    just the things we had before. In particular, it would seem that we need 
+    generators for the following:
+    - uid
+    - CFG
+    - Vminus states
+    - Vminus instructions
+    - values
+    But note again that the only value v (with cs', is) is computed by comp 
+    rather than generated, so we don't actually need a generator for value. 
+    Moreover, the CFG g should not be generated randomly the same way we do 
+    others, because it has to satisfy insns_at_pc; it is unlikely for just 
+    "any" CFG to satisfy this precondition of the lemma. *)
+
+(**
+    Exercise: Generators and Shows for uid and Vminus instructions, using 
+    automation as much as possible. (It is however useful to have custom Shows 
+    that are more descriptive.) *)
+
+(* FILL IN HERE *)
+
+(** For Vminus states, we already have a generator for mem. We have defined a 
+    generator and show for loc for you. *)
+
+Check gen_loc_from_atom_list.
+Check show_locals.
+
+(** Hence, write a generator and a show function for Vminus states, 
+    given domains for mem and loc. For simplicity, we can use the same 
+    domain for ploc. 
+ *)
+
+Definition gen_vminus_state
+           (mem_dom: list Atom.t)
+           (loc_dom: list Atom.t) : G state :=
+  (* FILL IN HERE *)
+       let gmem := gen_mem_from_atom_list mem_dom in
+       let gloc := gen_loc_from_atom_list mem_dom in
+       bindGen gmem (fun mem =>
+       bindGen arbitrary (fun pc =>
+       bindGen gloc (fun loc =>
+       bindGen arbitrary (fun ppc =>
+       bindGen gloc (fun prev_loc =>
+         returnGen
+           (mkst mem
+                 pc
+                 loc
+                 ppc
+                 prev_loc)))))).
+
+Definition show_vminus_state
+           (mem_dom: list Atom.t)
+           (loc_dom: list Atom.t)
+           (st: state) : string :=
+  (* FILL IN HERE *)
+  (show_memory (st_mem st) mem_dom ++ ", " ++
+               "pc: " ++ show (st_pc st) ++ ", " ++
+               show_locals (st_loc st) loc_dom ++ ", " ++
+               "ppc: " ++ show (st_ppc st) ++ ", " ++
+               "prev_loc: " ++ show_locals (st_ploc st) loc_dom)%string.
+
+(** With these out of the way, we can now address the remaining gaps. In its 
+    current form, comp_correct is inefficient and challenging for testing. 
+    Firstly, some of the quantities are computed by a function, so it is 
+    unnecessary to generate them in the first place, although seemingly 
+    suggested by "forall". Secondly, the CFG g is not just any CFG, but one 
+    that satisfies insns_at_pc for the compilation result - random generation 
+    in the usual way is very, very unlikely to meet this condition, so most
+    checks would end up being vacuously true. Thirdly, a Checker for the 
+    the existence of st' really needs to compute it, and this is not part of
+    the lemma itself. 
+
+    Hence the first order of affairs is to massage the lemma into a 
+    Checker-friendly version.
+ *)
+
+(** Firstly, let us drop the unnecessary variables, and note the generation 
+    of state.
+
+    Definition comp_correct (comp : ectmon (val * list insn))
+                            (eval : mem -> nat) : Prop :=
+      forall (cs: list uid) (g: ListCFG.t) (k: list insn),
+      forall (mem_dom: list Atom.t) (loc_dom: list Atom.t) (st: state),
+
+      let (cs', (v, is)) := comp cs in
+
+      insns_at_pc g (st_pc st) (is ++ k) ->
+      exists st',
+        st_mem st' = st_mem st /\
+        insns_at_pc g (st_pc st') k /\
+        star (Opsem.step g) st st' /\
+        ids_preserved cs st st' /\
+        good_return cs' v /\
+        ctx_incr cs cs' /\
+        eval_val (st_loc st') v = Some (eval (st_mem st)).
+
+    This is of course not accepted by Coq, but we will eventually get to a
+    Checker.
+ *)
+
+(** Secondly, we need to write a custom generator that generates CFGs 
+    satisfying insns_at_pc. An easier option is to just construct a CFG that 
+    loads the instructions at a given pc. 
+
+    Let us call this wrap_code_in_cfg' pc is k, in correspondence with 
+    insns_at_pc g (st_pc st) (is ++ k).
+
+    However, because pc may have a positive offset into the block, we should 
+    also fill the initial instructions with some dummy instructions (that won't
+    be executed). So make wrap_code_in_cfg' do this. 
+*)
+
+(* Returns a CFG with a single block containing instrs ++ instrs_after, 
+    and the pc in that block that begins at instrs_after *)
+Definition wrap_code_in_cfg' (p: pc) (instrs instrs_after: list insn)
+  : ListCFG.t :=
+  (* FILL IN HERE *)
+  let empty_cfg := [] in
+  let '(lbl, offset) := p in
+  let blocks :=
+      ListCFG.update empty_cfg lbl
+                     ((generate_dummy_insns offset)
+                        ++ instrs ++ instrs_after) in
+  (lbl, blocks).
+
+(** The to-be-Checkable lemma is thus:
+
+    Definition comp_correct (comp : ectmon (val * list insn))
+                            (eval : mem -> nat) : Prop :=
+      forall (cs: list uid) (k: list insn),
+      forall (mem_dom: list Atom.t) (loc_dom: list Atom.t) (st: state),
+
+      let (cs', (v, is)) := comp cs in
+      let g := wrap_code_in_cfg (st_pc st) is k in
+
+      exists st',
+        st_mem st' = st_mem st /\
+        insns_at_pc g (st_pc st') k /\
+        star (Opsem.step g) st st' /\
+        ids_preserved cs st st' /\
+        good_return cs' v /\
+        ctx_incr cs cs' /\
+        eval_val (st_loc st') v = Some (eval (st_mem st)). 
+*)
+
+(** Thirdly, if we have grasped the meaning of the lemma, we know that st'
+    is given by executing the compilation result; this is the point of 
+    "loading" the compilation result at the current pc in g, and is of course 
+    also stated by "star (Opsem.step g) st st'". So we need an executable 
+    evaluator for Vminus. The state st' is obtained by running this evaluator 
+    until we reach (the start of) k. 
+    
+    The simplest way of doing so is to stop at the program counter that begins
+    k, and this is actually determined by the CFG that loaded (is ++ k). 
+*)
+
+(** Exercise: Change wrap_code_in_cfg to return (g, pc), where the latter is 
+    the pc that begins k. *)
+
+Definition wrap_code_in_cfg (p: pc) (instrs instrs_after: list insn)
+  : ListCFG.t * pc :=
+  (* FILL IN HERE *)
+  let empty_cfg := [] in
+  let '(lbl, offset) := p in
+  let blocks :=
+      ListCFG.update empty_cfg lbl
+                     ((generate_dummy_insns offset)
+                        ++ instrs ++ instrs_after) in
+  ((lbl, blocks), (lbl, offset + List.length instrs)).
+
+(** Now we need the evaluator itself, which we have defined for you. *)
+
+Check V.Opsem.eval_until_pc.
+Check V.Opsem.eval_step.
+
+(** Now the lemma is:
+
+    Definition comp_correct (comp : ectmon (val * list insn))
+                            (eval : mem -> nat) : Prop :=
+      forall (cs: list uid) (k: list insn),
+      forall (mem_dom: list Atom.t) (loc_dom: list Atom.t) (st: state),
+
+      let (cs', (v, is)) := comp cs in
+      let (g, endpoint) := wrap_code_in_cfg (st_pc st) is k in
+
+      match V.Opsem.eval_until_pc g st cutpoint 1000 with
+      | inl err => false (* either out of fuel or no st' *)
+      | inr st' => 
+        st_mem st' = st_mem st /\
+        insns_at_pc g (st_pc st') k /\
+        star (Opsem.step g) st st' /\
+        ids_preserved cs st st' /\
+        good_return cs' v /\
+        ctx_incr cs cs' /\
+        eval_val (st_loc st') v = Some (eval (st_mem st))
+      end.
+ *)
+
+(** And with this, the major obstacles are out of the way, and we only have
+    to write a Checker for the big conjunction. Because the conjunction is 
+    huge, it is easier to write a Checker for each conjunct. That is, we would
+    like to have:
+    - A Checker that checks that two memories are the same. This has already 
+      been done.
+    - A Checker that checks for insns_at_pc g.
+    - A Checker for ids_preserved.
+    - A Checker for good_return.
+    - A Checker for ctxt_incr.
+    - A Checker that checks for equality between the two ways of evaluation.
+    Note that "star (Opsem.step g) st st'" doesn't need checking, because it is
+    implicit in eval_until_pc. With respect to correctness of aexp compilation 
+    itself, the last is most relevant. 
+
+    To give a headstart, most of these are defined below.
+*)
+
+Fixpoint loc_on_domain_checker
+         (dom: list uid) (loc1 loc2 : loc) : Checker :=
+  match dom with
+  | [] => checker true
+  | (a :: l) =>
+    match loc1 a, loc2 a with
+    | Some n1, Some n2 =>
+      if Nat.eqb n1 n2 then loc_on_domain_checker l loc1 loc2
+      else whenFail "loc_equal: locs disagree" false
+    | None, None => loc_on_domain_checker l loc1 loc2
+    | _, _ => whenFail "loc_equal: locs disagree" false
+    end
+  end.
+
+Fixpoint insns_at_pc_checker `{Show pc}
+         (g: ListCFG.t) (p: pc) (k : list insn) : Checker :=
+  match k with
+  | [] => checker true
+  | (uid, cmd) :: instrs =>
+    match ListCFG.fetch g p with
+    | Some (uid', cmd') =>
+      if eq_dec_uid uid uid' then
+        if eq_dec_cmd cmd cmd' then insns_at_pc_checker g (incr_pc p) instrs
+        else whenFail ("insns_at_pc: cmd at pc "
+                         ++ (show p) ++ " not equal") false
+      else whenFail ("insns_at_pc: uid at pc "
+                       ++ (show p) ++ "not equal") false
+    | None => whenFail "insns_at_pc: cannot fetch" false
+    end
+  end.
+
+Definition eval_equal_checker (eval: mem -> nat) (st: state) (v: val)
+  : Checker :=
+  let run_result := eval_val (st_loc st) v in
+  let expected_result := eval (st_mem st) in
+  match run_result with
+  | Some n =>
+    whenFail "eval_equal: evaluation value not the same"
+             (Nat.eqb n expected_result)
+  | None => whenFail "eval_equal: run did not obtain any value" false
+  end.
+
+Definition ids_preserved_checker (cs : list uid) (st st': state)
+  : Checker :=
+  loc_on_domain_checker cs (st_loc st) (st_loc st').
+
+
+Definition good_return_checker (cs: list uid) (v: val) : Checker :=
+  match v with
+  | val_uid uid =>
+    whenFail "good_return: cannot find value" 
+             (List.existsb
+                (fun uid' => if eq_dec_uid uid uid' then true else false) cs)
+  | val_nat n => checker true
+  end.
+
+Fixpoint ctx_incr_checker (cs cs': list uid) : Checker :=
+  (* FILL IN HERE *)
+  match cs with
+  | [] => checker true
+  | (uid :: uids) =>
+    if (List.existsb
+          (fun uid' => if eq_dec_uid uid uid' then true else false) cs') then
+      ctx_incr_checker uids cs'
+    else whenFail ("ctx_incr: " ++ show uid ++ " not found") false
+  end.
+
+(** We can now compose the checkers using QuickChick's conjoin combinator. *)
+Definition expression_step_checker
+           (eval: V.Opsem.mem -> nat)
+           (g: ListCFG.t)
+           (initial_state final_state: V.Opsem.state)
+           (k: list insn) (end_of_expr: pc)
+           (cs cs': list uid)
+           (v : val) : Checker :=
+  conjoin [ids_preserved_checker cs initial_state final_state;
+             insns_at_pc_checker g end_of_expr k;
+             good_return_checker cs' v;
+             ctx_incr_checker cs cs';
+             eval_equal_checker eval final_state v].
+
+(** Finally, a Checker for comp_correct and comp_aexp could look like the 
+    following. It is convenient to split the Checker into a part that does 
+    only the generation, and a part that does the checking, because a type 
+    error can cause the typechecker to get stuck trying to resolve the issue
+    by looking for typeclass instances that don't exist.    
+*)
+
+Definition comp_correct_checker_inner
+           (comp: ectmon (val * list insn)) (eval: V.Opsem.mem -> nat)
+           (cs : list uid) (st: V.Opsem.state) (k: list insn)
+  : Checker :=
+  let '(cs', (v, instrs)) := comp cs in
+  let '(g, endpoint) := wrap_code_in_cfg (V.Opsem.st_pc st) instrs k in
+  match V.Opsem.eval_until_pc g st endpoint 1000 with
+  | inl err => whenFail ("comp_correct_checker: " ++ err) false
+  | inr st' => 
+    expression_step_checker eval g st st' k endpoint cs cs' v
+  end.
+
+Definition comp_correct_checker
+           (comp: ectmon (val * list insn)) (eval: V.Opsem.mem -> nat)
+  : Checker :=
+  forAll arbitrary (fun (cs : list uid) =>
+  forAll arbitrary (fun (extra_insn : list insn) =>
+  forAll arbitrary (fun (mem_dom: list Atom.t) =>
+  forAll arbitrary (fun (loc_dom: list Atom.t) =>
+  forAllShrinkShow (gen_vminus_state mem_dom loc_dom)
+                   (fun x => [])
+                   (show_vminus_state mem_dom loc_dom)
+                   (fun (start_state: state) => 
+    comp_correct_checker_inner
+      comp eval
+      cs start_state extra_insn))))).
+
+(**! Section test_compile_aexp extends compiler *)
+
+Definition comp_aexp_correct_checker :=
+  forAll arbitrary (fun a: aexp =>
+    (* collect a ( *) comp_correct_checker (comp_aexp a) (aeval a)).
+
+(* ! QuickChick comp_aexp_correct_checker. *)
+
+(** Since the compiler has already been proven correct, all tests should 
+    succeed. However, they could be succeeding for rather vacuous reasons, and 
+    it would be assuring to know that the Checker indeed fails when the 
+    compiler is wrong. 
+
+    Exercise: Add mutants to comp_aexp, and verify that they are causing 
+    comp_aexp_correct_checker to fail. 
+ *)
+
+(** Exercise: Write a Checker for the following lemma, and run it.
+
+Lemma comp_bop_correct : forall b comp1 comp2 eval1 eval2
+    (IHa1: comp_correct comp1 eval1)
+    (IHa2: comp_correct comp2 eval2),
+    comp_correct (comp_bop b comp1 comp2)
+                 (fun m => bop_denote b (eval1 m) (eval2 m)).
+ *)
+
+Definition comp_bop_correct_checker: Checker :=
+  (* FILL IN HERE *)
+  forAll arbitrary (fun (a1: aexp) =>
+  forAll arbitrary (fun (a2: aexp) =>
+  forAll arbitrary (fun (binop: bop) => 
+    collect binop (comp_correct_checker 
+      (comp_bop binop (comp_aexp a1) (comp_aexp a2))
+      (fun m => V.Opsem.bop_denote binop (aeval a1 m) (aeval a2 m)))))).
+
+(* ! QuickChick comp_bop_correct_checker. *)
+
+Definition comp_bexp_correct_checker : Checker :=
+  forAll arbitrary (fun b: bexp => 
+    comp_correct_checker (comp_bexp b) (fun m => if (beval b m) then 1 else 0)).
+
+(* ! QuickChick comp_bexp_correct_checker. *)
+
+(** Exercise: Write a Checker for the following lemma, and make sure that all 
+    tests pass. 
+
+Lemma comp_bexp_correct : forall (b:bexp),
+  comp_correct (comp_bexp b) (fun m => b2n (beval b m)).
+*)
+
+(** Exercise: Write a Checker for the following lemma, and make sure that all 
+    tests pass.
+
+Lemma comp_store_correct : 
+  forall g a v le lr cs st,
+  insns_at_pc g (block_entry le) (steval (comp_store a v lr) cs) ->
+  st_pc st = (block_entry le) ->
+  exists st',
+    plus (step g) st st' /\
+    st_pc st' = (block_entry lr) /\
+    st_mem st' = (Memory.update (st_mem st) v (aeval a (st_mem st))).
+ *)
+
+Definition comp_store_correct_checker_inner
+           (a : aexp) (v: addr) (lr le: lbl) (cs: list uid)
+           (mem_dom: list Atom.t) (loc_dom: list Atom.t) (vst: state)
+  : Checker :=
+  (* FILL IN HERE *)
+  let st := mkst (st_mem vst) (block_entry le) (st_loc vst)
+                 (st_ppc vst) (st_ploc vst) in
+  let '(g, end_pc) :=
+      wrap_code_in_cfg (block_entry le)
+                       (steval (comp_store a v lr) cs) [] in
+  match (V.Opsem.eval_once_and_until_pc g st (block_entry lr) 1000) with
+  | inl err => whenFail ("comp_store_correct: " ++ err) false
+  | inr st' =>
+    if (eq_dec_pc (V.Opsem.st_pc st') (block_entry lr)) then
+      let new_dom := (v :: mem_dom) in
+      whenFail 
+        "comp_store_correct: memories mismatch"
+        (memory_on_domain_checker new_dom
+          (V.Opsem.st_mem st')
+          (V.Opsem.Memory.update (V.Opsem.st_mem st) v
+                                 (aeval a (V.Opsem.st_mem st))))
+    else whenFail "comp_store_correct: pc not expected" false
+  end.
+
+Definition comp_store_correct_checker: Checker :=
+  forAll arbitrary (fun (a: aexp) =>
+  forAll arbitrary (fun (v: addr) =>
+  forAll arbitrary (fun (lr: lbl) =>
+  forAll arbitrary (fun (le: lbl) =>
+  forAll arbitrary (fun (cs: list uid) =>
+  forAll arbitrary (fun (mem_dom: list Atom.t) =>
+  forAll arbitrary (fun (loc_dom: list Atom.t) =>
+  forAllShrinkShow (gen_vminus_state mem_dom loc_dom)                      
+                   (fun x => [])
+                   (show_vminus_state mem_dom loc_dom)
+                   (fun (vst: state) => 
+    comp_store_correct_checker_inner a v lr le cs mem_dom loc_dom vst)))))))).
+
+
+(** Exercise: Write a Checker for the following lemma, and make sure that all 
+    tests pass.
+
+Lemma comp_cond_correct :
+  forall g cs b le l1 l2 st,
+  insns_at_pc g (block_entry le) (steval (comp_cond b l1 l2) cs) ->
+  st_pc st = (block_entry le) ->
+  exists st',
+    plus (step g) st st' /\
+    st_pc st' = block_entry (if beval b (st_mem st) then l1 else l2) /\
+    st_mem st = st_mem st'.
+*)
+
+Definition comp_cond_correct_checker_inner
+           (b: bexp) (cs: list uid) (le l1 l2: lbl)
+           (mem_dom: list Atom.t) (loc_dom: list Atom.t) (vst: state)
+  : Checker :=
+  (* FILL IN HERE *)
+  let st := mkst (st_mem vst) (block_entry le) (st_loc vst)
+                 (st_ppc vst) (st_ploc vst) in
+  let '(g, end_pc) :=
+      wrap_code_in_cfg (block_entry le)
+                       (steval (comp_cond b l1 l2) cs) [] in
+  let l := (if beval b (V.Opsem.st_mem st) then l1 else l2) in  
+  match (V.Opsem.eval_until_pc g st (block_entry l) 1000) with
+  | inl err =>
+    whenFail 
+      ("::: cfg is: " ++ show g ++
+       "::: comp_cond_correct: " ++ err ++
+       "::: looking for pc: " ++ show end_pc
+      )
+      false
+  | inr st' =>
+    if (eq_dec_pc (V.Opsem.st_pc st') (block_entry l)) then 
+      whenFail "comp_store_correct: memories mismatch"
+               (memory_on_domain_checker mem_dom
+                                         (st_mem st)
+                                         (st_mem st'))
+    else whenFail "comp_cond_correct: pc not expected" false
+  end.
+
+Definition comp_cond_correct_checker : Checker :=
+  forAll arbitrary (fun (b: bexp) =>
+  forAll arbitrary (fun (le: lbl) =>
+  forAll arbitrary (fun (l1: lbl) =>
+  forAll arbitrary (fun (l2: lbl) =>
+  forAll arbitrary (fun (cs: list uid) =>
+  forAll arbitrary (fun (mem_dom: list Atom.t) =>
+  forAll arbitrary (fun (loc_dom: list Atom.t) =>
+  forAllShrinkShow (gen_vminus_state mem_dom loc_dom)                      
+                   (fun x => [])
+                   (show_vminus_state mem_dom loc_dom)
+                   (fun (vst: state) => 
+    comp_cond_correct_checker_inner b cs le l1 l2 mem_dom loc_dom vst)))))))).
+
+(* ! QuickChick comp_cond_correct_checker. *)
