vminus/Dom.v
@@ -1,0 +1,168 @@
+(* -------------------------------------------------------------------------- *
+ *                     Vellvm - the Verified LLVM project                     *
+ *                                                                            *
+ *     Copyright (c) 2017 Steve Zdancewic <stevez@cis.upenn.edu>              *
+ *                                                                            *
+ *   This file is distributed under the terms of the GNU General Public       *
+ *   License as published by the Free Software Foundation, either version     *
+ *   3 of the License, or (at your option) any later version.                 *
+ ---------------------------------------------------------------------------- *)
+
+Require Import List Equalities Orders RelationClasses.
+Require Import FSets FMaps.
+Import ListNotations.
+Require Import Util.
+
+(* ################################################################# *)
+(** * Dom: Reasoning about dominators in a graph. *)
+
+
+(* ################################################################# *)
+(** * GRAPH *)
+(** Interface for a nonempty graph [t] with: 
+     - a set of _vertices_ of type [V], defined by a membership predicate [Mem]
+     - a distinguished _entry vertex_ [entry]
+     - an _edge relation_ [Succ]
+*)
+
+Module Type GRAPH.
+  Parameter Inline t V : Type.
+  
+  Parameter Inline entry : t -> V.
+  Parameter Inline Succ : t -> V -> V -> Prop.
+  Parameter Inline Mem : t -> V -> Prop.
+End GRAPH.
+
+(**  ------------------------------------------------------------------------- *)
+(* ################################################################# *)
+(** * Specification of Dominators *)
+
+(** This is a relational specification of the graph dominance properties that 
+    is convenient for proofs and intuitively captures the definitions. *)
+
+Module Spec (Import G:GRAPH).
+
+(** We first define a _path_ in the graph.
+
+    [path g v1 v2 vs] means that there is a sequence of vertices
+    starting from vertex [v1] and ending at [v2] that are connected by
+    the [Succ] relation.  The vertices traversed on the path are those
+    listed in [vs] (in reverse order).  
+*)
+
+  Inductive Path (g:G.t) : V -> V -> list V -> Prop :=
+  | path_nil : forall v, 
+      Mem g v -> Path g v v [v]
+  | path_cons : forall v1 v2 v3 vs,
+      Path g v1 v2 vs -> Mem g v3 -> Succ g v2 v3 
+      -> Path g v1 v3 (v3::vs).
+
+(**  ------------------------------------------------------------------------- *)  
+(* ----------------------------------------------------------------- *)
+(** *** Definition of domination *)
+
+  (** Vertex [v1] _dominates_ vertex [v2] if every path starting 
+      from the entry of the graph and ending at [v2] goes through [v1]. *)
+  
+  Definition Dom (g:G.t) (v1 v2: V) : Prop :=
+    forall vs, Path g (entry g) v2 vs -> In v1 vs.
+
+  (** Vertex [v1] _strictly dominates_ [v2] if they are distinct and 
+     [v1] dominates [v2] *)
+  
+  Definition SDom (g:G.t) (v1 v2 : V) : Prop :=
+    v1 <> v2 /\ Dom g v1 v2.
+
+
+(**  ------------------------------------------------------------------------- *)  
+(* ----------------------------------------------------------------- *)
+(** *** Interaction of dominance and Succ *)
+
+  (** The strict dominators of a vertex [v2] also dominate its predecessors. *)
+  
+  Lemma dom_step : forall g v1 v2,
+    Mem g v2 -> Succ g v1 v2 -> forall v', SDom g v' v2 -> Dom g v' v1.
+  Proof.
+    unfold SDom, Dom. intros g v1 v2 Hmem Hsucc v' [Hneq Hdom] p Hp.
+    cut (In v' (v2::p)). inversion 1; subst; intuition. 
+    apply Hdom. eapply path_cons; eauto. 
+  Qed.
+
+End Spec.
+
+(**  ------------------------------------------------------------------------- *)  
+(* ################################################################# *)
+(** * Computing Dominance Properties *)
+
+(** As usual, if we want to run the dominance calculation, we need an executable
+    version of the specification.  For dominance, we can think of an implementation
+    as an function that takes a graph and produces a mapping that sends each
+    vertex to its set of strict dominators.  Any correct implementation must be sound 
+    (and complete) with respect to the relational spec defined above.  This 
+    interface capture the requirements of such an implementation.
+
+    Full soundness follows from an "unrolled" version of the [dom_step] property.
+*)
+
+Module Type Algdom (Import G:GRAPH).
+  Module Import GS := Spec G.
+
+  Declare Module E : UsualDecidableType with Definition t := V.
+  Declare Module NS : FSetInterface.WS with Module E:=E.
+  Module L := BoundedSet NS.
+  Include EqLeNotation L.
+
+  Parameter calc_sdom : G.t -> option (V -> L.t).
+
+  Axiom entry_sound : forall g sdom,
+    calc_sdom g = Some sdom ->
+    sdom (entry g) == L.top.
+
+  Axiom successors_sound : forall g sdom n1 n2,
+    calc_sdom g = Some sdom ->
+    Mem g n1 -> Mem g n2 -> Succ g n1 n2 -> 
+    L.union (L.singleton n1) (sdom n1) <= sdom n2.
+
+  Axiom complete : forall g sdom n1 n2,
+    calc_sdom g = Some sdom ->
+    SDom g n1 n2 -> L.In n1 (sdom n2).
+
+End Algdom.
+
+(**  ------------------------------------------------------------------------- *)  
+(* ################################################################# *)
+(** * Full Soundness *)
+
+(** The full soundness result follows as a corollary of the [entry_sound] and
+    [successors_sound] properties of [Algdom].
+*)
+
+Module AlgdomProperties (Import G:GRAPH) (Import A : Algdom G).
+  Module Import GS := Spec G.
+
+  Lemma sound : forall g sdom n1 n2,
+    calc_sdom g = Some sdom ->              
+    L.In n1 (sdom n2) -> Dom g n1 n2.
+  Proof.
+    red; intros. remember (entry g). induction H1. subst.
+    pose proof entry_sound g sdom H. 
+
+    destruct (sdom (entry g)); try contradiction; simpl in *.
+      exfalso. rewrite H2 in H0. eapply L.SFacts.empty_iff. eauto.
+      
+    right. destruct (E.eq_dec v2 n1). subst. inversion H1; intuition.
+    apply IHPath; auto.
+
+    destruct (sdom v2) eqn:Heqv2; simpl in *; auto.
+    cut (NS.In n1 (NS.union (NS.singleton v2) t0)).
+    intro Hin. apply NS.union_1 in Hin as [Hin | Hin]; auto.
+    contradict n. apply NS.singleton_1. assumption.
+
+    pose proof successors_sound g sdom v2 v3 as Hss.
+    simpl in Hss. rewrite Heqv2 in Hss. simpl in Hss.
+    destruct (sdom v3). apply Hss; inversion H1; eauto.
+    exfalso. apply Hss; inversion H1; eauto.
+  Qed.
+
+End AlgdomProperties.
+
