vminus/Vminus.v
@@ -1,0 +1,234 @@
+(** * Vminus: A Simple SSA Intermediate Representation *)
+
+(** This file defines the syntax and semantics for Vminus, an
+    intermediate representation that is intended to capture the
+    essence of LLVM's IR.  In particular, this language represents
+    code as a _control flow graph_ whose blocks contain instructions
+    in _static single assignment_ form.  This means that each
+    instruction _defines_ (at most) one local identifier and that
+    those identifiers are _immutable_.  To make this work in practice,
+    SSA representations introduce the notation of _phi functions_,
+    whose value is determined by the run-time control flow of the
+    program.
+
+    To support mutable state, Vminus also has Imp-style global
+    identifiers.
+*)
+
+Require Import Arith List.
+Import ListNotations.
+
+Require Import Vminus.Classes Vminus.Atom Vminus.Util.
+
+
+Instance eq_dec_atom : eq_dec Atom.t := Atom.eq_dec.
+Hint Resolve eq_dec_atom.
+Hint Resolve Atom.eq_dec.
+Hint Resolve eq_nat_dec.
+
+(**  ------------------------------------------------------------------------- *)
+(* ################################################################# *)
+(** * Vminus labels, identifiers, and addresses.  *)
+
+
+(** Basic block labels *)
+
+Module Lbl := Atom.
+Notation lbl := Lbl.t.
+
+(** Local unique identifiers *)
+
+Module Uid := Atom.
+Notation uid := Uid.t.
+
+(** Addresses of mutable state *)
+
+Module Addr := Atom. 
+Notation addr := Addr.t.
+
+(** All come equipped with decidable equality. *)
+
+Definition eq_dec_lbl : forall l1 l2, {l1 = l2} + {l1 <> l2} := Atom.eq_dec.
+Hint Resolve eq_dec_lbl.
+
+Definition eq_dec_uid : forall u1 u2, {u1 = u2} + {u1 <> u2} := Atom.eq_dec.
+Hint Resolve eq_dec_uid.
+
+Definition eq_dec_addr : forall a1 a2, {a1 = a2} + {a1 <> a2} := Atom.eq_dec.
+Hint Resolve eq_dec_addr.
+
+
+(**  ------------------------------------------------------------------------- *)
+(* ################################################################# *)
+(** * Values and Binary Operations *)
+
+(** Values are just local identifiers or natural numbers *)
+
+Inductive val : Set :=
+ | val_uid  : uid -> val
+ | val_nat : nat -> val.
+
+Definition eq_dec_val : forall (v1 v2:val) , {v1 = v2} + {v1 <> v2}.
+Proof.
+  decide equality.
+Defined.
+Instance eq_val : eq_dec val := eq_dec_val.
+Hint Resolve eq_dec_val.
+
+
+(** All Vminus operations are binary arithmetic forms.  There are no
+    unary operations, nor are there assembly-language-like [move]
+    instructions.
+*)
+
+Inductive bop : Set := 
+ | bop_add   (* addition *)
+ | bop_sub   (* subtraction *)
+ | bop_mul   (* multiplication *)
+ | bop_eq    (* equality *)
+ | bop_le    (* less-than-or-equal *)
+ | bop_and   (* both non-zero *)
+.  
+
+Definition eq_dec_bop : forall (b1 b2:bop), {b1 = b2} + {b1 <> b2}.
+Proof.
+  decide equality.
+Defined.
+Instance eq_bop : eq_dec bop := eq_dec_bop.
+Hint Resolve eq_dec_bop.
+
+
+(**  ------------------------------------------------------------------------- *)
+(* ################################################################# *)
+(** * Basic block terminators *)
+
+(** Each basic block is a sequence of commands (defined next) ending
+    in a _terminator_, which is just a control flow operation.  
+    Terminators cannot appear in the middle of a well-formed basic block.
+    (We will define well-formed Vminus programs later.)
+*)
+
+Inductive tmn : Set :=
+| tmn_jmp : lbl -> tmn                  (* unconditional jump *)
+| tmn_cbr : val -> lbl -> lbl -> tmn    (* conditional branch *)
+| tmn_ret : tmn.                        (* return *)
+
+Definition eq_dec_tmn : forall (t1 t2:tmn), {t1 = t2} + {t1 <> t2}.
+Proof.
+  decide equality.
+Defined.
+Instance eq_tmn : eq_dec tmn := eq_dec_tmn.
+Hint Resolve eq_dec_tmn.
+
+(**  ------------------------------------------------------------------------- *)
+(* ################################################################# *)
+(** * Commands *)
+
+(** Vminus has only a few commands: binary operations, 
+    terminators, phi nodes, and [load] and [store] operations. *)
+
+(** Each [phiarg] associates a value with a predessor block, given by
+    a [lbl]. *)
+
+Definition phiarg := (lbl * val)%type.
+
+Definition eq_dec_phiarg:
+  forall phiarg1 phiarg2: phiarg, {phiarg1 = phiarg2} + {phiarg1 <> phiarg2}.
+Proof.
+  decide equality.
+Defined.  
+Instance eq_phiarg : eq_dec phiarg := eq_dec_phiarg.
+Hint Resolve eq_dec_phiarg.
+
+Definition eq_dec_list_phiarg:
+  forall l1 l2 : list phiarg, {l1 = l2} + {~(l1 = l2)}.
+Proof.
+  decide equality.
+Defined.
+Hint Resolve eq_dec_list_phiarg.
+    
+(** Vminus Commands *)
+
+Inductive cmd : Set :=
+| cmd_bop   : bop -> val -> val -> cmd
+| cmd_phi   : list phiarg -> cmd
+| cmd_tmn   : tmn -> cmd
+| cmd_load  : addr -> cmd
+| cmd_store : addr -> val -> cmd.
+
+Definition eq_dec_cmd: forall cmd1 cmd2: cmd, {cmd1 = cmd2} + {~(cmd1 = cmd2)}.
+Proof.
+  decide equality.
+Defined.  
+Instance eq_cmd : eq_dec cmd := eq_dec_cmd.
+Hint Resolve eq_dec_cmd.
+
+(** An instruction associates a unique local identifier with one of the
+    above commands. The local identifier serves two purposes:
+
+    - it uniquely identifies this occurrence of the command 
+    - it serves as the value 
+
+
+*)
+
+Definition insn := (uid * cmd)%type.
+
+Definition eq_dec_insn:
+  forall insn1 insn2: insn, {insn1 = insn2} + {~(insn1 = insn2)}.
+Proof.
+  decide equality.
+Defined. 
+Instance eq_insn : eq_dec insn := eq_dec_insn.
+Hint Resolve eq_dec_insn.
+
+(**  ------------------------------------------------------------------------- *)
+(* ----------------------------------------------------------------- *)
+(** *** Useful predicates about instructions *)
+
+(** Which values are used by an instruction? *)
+Definition insn_uses (i:insn) : list val :=
+  match i with
+    | (_, cmd_bop _ v1 v2) => [v1; v2]
+    | (_, cmd_phi pas) => map (@snd _ _) pas
+    | (_, cmd_tmn (tmn_cbr v _ _)) => [v]
+    | (_, cmd_store _ v) => [v]
+    | (_, _) => []
+  end.
+
+(** Which labels appear in an instruction? *)
+Definition insn_lbls (i:insn) : list lbl :=
+  match i with 
+    | (_, cmd_tmn (tmn_jmp l)) => [l]
+    | (_, cmd_tmn (tmn_cbr _ l1 l2)) => [l1; l2]
+    | _ => []
+  end.
+
+(** Which phi arguments appear in an instruction? *)
+Definition insn_phis (i:insn) : list phiarg :=
+  match i with
+    | (_, cmd_phi pas) => pas
+    | _ => []
+  end.
+
+(** Is it a terminator? *)
+Definition is_tmn (i:insn) : Prop := 
+  match i with (_, cmd_tmn _) => True | _ => False end.
+
+(** Is is a phi node? *)
+Definition is_phi (i:insn) : Prop := 
+  match i with (_, cmd_phi _) => True | _ => False end.
+
+Lemma is_phi_decidable : forall i, {is_phi i} + {~is_phi i}.
+Proof.
+  intros [? c].
+  destruct c; simpl; tauto.
+Qed.  
+
+(** Does it define its uid? *)
+Definition defs_uid (i:insn) : Prop :=
+  match i with
+    | (_, cmd_tmn _) | (_, cmd_store _ _) => False | _ => True
+  end.
+
+
