vminus/VminusOpSem.v
@@ -1,0 +1,391 @@
+Require Import Arith.
+Require Import List.
+Import ListNotations.
+Require Import String.
+
+Require Import Vminus.Classes.
+Require Import Vminus.Util.
+Require Import Vminus.Env.
+Require Import Vminus.Vminus.
+Require Import Vminus.CFG.
+
+
+
+(* ################################################################# *)
+(** * Vminus Operational Semantics *)
+
+(** This file provides both relational and executable definitions of
+    the Vminus operational semantics and proves them equivalent.
+
+    We can reason about the semantics of Vminus programs using only
+    the relational specification, but if we want to _test_ them or
+    extract an interpreter, we need to have the executable version
+    too.  Once we have established that the two semantics correspond,
+    it is easy to prove that the relational semantics is deterministic
+    because it is equivalent to the executable semantics, which is
+    given by a function.  
+    
+    The development is parameterized by a control-flow graph, making
+    the operational semantics independent of its representation.
+
+    Later, as a demonstration of using these semantics, we will prove
+    the correctness of an Imp to Vminus compiler and some program  
+    transformations as the Vminus level.
+*)
+
+
+
+Module Make (Cfg:CFG).
+Import Cfg.
+
+Module Opsem.
+  (**  ------------------------------------------------------------------------- *)
+  (** *** The state of a Vminus program: *)
+
+  (** The local environment is a _partial_ map from [uid]s to 
+      natural numbers. *)
+  
+  Module Locals := Make_Env(Uid).
+  Notation loc := (Locals.t (option nat)).
+  Notation update := Locals.update.
+
+  (** The Vminus memory is a _total_ map from addresses to 
+      natural numbers.  (This is a bit artificial, but is a simplification 
+      that aligns with the variant of Imp we use in this development.)
+  *)
+
+  Module Memory := Make_Env(Addr).
+  Notation mem := (Memory.t nat).
+
+  (** The state packages together the memory, local environment,
+      current program counter.  It also remembers the environment
+      in effect at the end of the of the predecessor block, for
+      use in phi instructions (see below). *)
+  
+  Record state := mkst { st_mem  : mem
+                       ; st_pc   : pc
+                       ; st_loc  : loc
+                       ; st_ppc  : pc     (* predecessor pc *)
+                       ; st_ploc : loc    (* predecessor locals *) 
+                       }.
+
+  (**  ------------------------------------------------------------------------- *)
+  (** *** Evaluating values. *)
+
+  (** Simply look up the uid in the local environment. (May fail!) *)
+  
+  Definition eval_val (loc:loc) (v:val) : option nat :=
+    match v with
+      | val_nat n => Some n
+      | val_uid i => loc i
+    end.
+
+  (**  ------------------------------------------------------------------------- *)
+  (** *** Evaluating binary operations. *)
+
+  Definition b2n (b:bool) := if b then 1 else 0.
+  Definition n2b (n:nat) := if n then false else true.
+
+  Definition bop_denote (bop:bop) : nat -> nat -> nat :=
+    match bop with
+      | bop_add => plus
+      | bop_sub => minus
+      | bop_mul => mult
+      | bop_eq => fun n m => b2n (beq_nat n m)
+      | bop_le => fun n m => b2n (leb n m)
+      | bop_and => fun n m => b2n (n2b n && n2b m)
+    end.
+
+  Definition eval_bop (loc:loc) (bop:bop) (v1 v2:val) : option nat :=
+    match eval_val loc v1, eval_val loc v2 with
+      | Some n1, Some n2 => Some (bop_denote bop n1 n2) 
+      | _, _ => None
+    end.
+
+  (**  ------------------------------------------------------------------------- *)
+  (** *** Evaluating phi nodes *)
+  (** To evaluate a phi instruction, we need to know from which 
+      predecessor block control reached this phi node, as well as
+      the local environment in effect at the end of that block.
+      
+      We look up the value associated with the predecessor label 
+      in the phi arg list, and interpret it in the predecessor's 
+      local environment, which are supplied to [eval_phi].
+  *)
+
+  Definition eval_phi (ploc:loc) (pl:lbl) (pas:list phiarg) 
+    : option nat :=
+    match assoc Lbl.eq_dec pl pas with
+      | Some v => eval_val ploc v
+      | None => None
+    end.
+
+  (**  ------------------------------------------------------------------------- *)
+  (** *** Control transfers *)
+  
+  (** Given the current locals and the terminator, determine
+      the label of the next block to jump to (if any). *)
+
+  Definition eval_tmn (loc:loc) (t:tmn) : option lbl :=
+    match t with
+      | tmn_jmp l => Some l
+      | tmn_cbr v l1 l2 =>
+          match eval_val loc v with
+            | Some n => Some (if n then l2 else l1)
+            | None => None
+          end
+      | _ => None
+    end.
+
+  (**  ------------------------------------------------------------------------- *)
+  (** *** Small-step, relational operational semantics *)
+
+  Inductive step (g:Cfg.t) : state -> state -> Prop :=
+
+  | step_bop : forall mem pc loc bop v1 v2 uid n ppc ploc,
+      insn_at_pc g pc (uid, cmd_bop bop v1 v2) ->
+      Some n = eval_bop loc bop v1 v2 ->
+      step g (mkst mem pc loc ppc ploc) 
+             (mkst mem (incr_pc pc) 
+                       (update loc uid (Some n)) ppc ploc)
+
+  (** Evaluate the right-hand side in the predecessor's 
+     local environment. [lbl_of ppc] is the source block of the 
+     control-flow edge that we jumped from to reach the current block. *)
+
+  | step_phi : forall mem pc loc pas uid n ppc ploc,
+      insn_at_pc g pc (uid, cmd_phi pas) ->
+      Some n = eval_phi ploc (lbl_of ppc) pas ->
+      step g (mkst mem pc loc ppc ploc)
+             (mkst mem (incr_pc pc) 
+                       (update loc uid (Some n)) ppc ploc)
+
+  (** Find the successor block (if any), update the pc. 
+      Record the current pc and locals as the "predecessor" state
+      for use by any [phi] nodes in the successor block. *)
+
+  | step_tmn : forall mem pc l' loc tmn uid ppc ploc, 
+      insn_at_pc g pc (uid, cmd_tmn tmn) ->
+      Some l' = eval_tmn loc tmn ->
+      step g (mkst mem pc loc ppc ploc)
+             (mkst mem (block_entry l') loc pc loc)
+
+  (** Loads and stores simply read from/write to the memory component of the state. **)
+
+  | step_load : forall mem pc loc uid addr ppc ploc,
+      insn_at_pc g pc (uid, cmd_load addr) ->
+      step g (mkst mem pc loc ppc ploc)
+             (mkst mem (incr_pc pc) 
+                       (update loc uid (Some (mem addr))) ppc ploc)
+
+  | step_store : forall mem pc loc uid addr v n ppc ploc,
+      insn_at_pc g pc (uid, cmd_store addr v) ->
+      Some n = eval_val loc v ->
+      step g (mkst mem pc loc ppc ploc)
+             (mkst (Memory.update mem addr n) 
+                   (incr_pc pc) loc ppc ploc).
+
+
+ (**  ------------------------------------------------------------------------- *)
+ (** *** Definition of the initial state. *)
+
+ (** The initial state starts with the program counter at the beginning of the
+     entry block in an empty environment.  The "predecessor state" can be 
+     set arbitrarily -- we will prove that in any well-formed CFG, the 
+     entry block cannot have any phi nodes. *)
+  
+  Definition init_state (g:Cfg.t) (m: mem) : state :=
+    (mkst m
+          (block_entry (entry_block g))
+          (Locals.empty None)
+          (block_entry (entry_block g))
+          (Locals.empty None)).
+
+
+  (**  ------------------------------------------------------------------------- *)  
+  (** * Small-step, executable operational semantics *)
+
+  (** This version of the semantics is just a straight forward interpreter, 
+      implemented monadically in an error monad to deal with partiality. 
+       
+      It uses [fetch] where the relational specification uses [insn_at_pc], but
+      is otherwise a fairly direct transliteration of the relational version.
+
+      Note: the monad notation and definitions come from [Classes.v], a 
+      general purpose library that collects together some commonly used
+      typeclasses and instances.
+
+      - [mret] is the "return" of a monad    
+      - the notation  ['x <- e1; e2] is the "bind"
+      - [trywith] lifts the [option] monad into the [err] monad
+  *)
+  (**  ------------------------------------------------------------------------- *)  
+  
+  Fixpoint eval_step (g : Cfg.t) (s : state) : err state :=
+    let 'mkst mem pc loc ppc ploc := s in
+    '(uid, insn) <- trywith "no instruction fetched" (Cfg.fetch g pc); 
+    match insn with
+    | cmd_bop bop v1 v2 =>    
+      'n <- trywith "cannot evalute binop command"  (eval_bop loc bop v1 v2);
+      mret (mkst mem (incr_pc pc) (update loc uid (Some n)) ppc ploc)
+
+    | cmd_phi pas =>
+      'n <- trywith "cannot evaluate phi" (eval_phi ploc (lbl_of ppc) pas);
+      mret (mkst mem (incr_pc pc) (update loc uid (Some n)) ppc ploc)
+           
+    | cmd_tmn tmn =>
+      'l' <- trywith "cannot evaluate terminator" (eval_tmn loc tmn);
+      mret (mkst mem (block_entry l') loc pc loc)
+
+    | cmd_load addr =>
+      mret (mkst mem (incr_pc pc) (update loc uid (Some (mem addr))) ppc ploc)
+
+    | cmd_store addr v =>
+      'n <- trywith "cannot evaluate address to store to" (eval_val loc v);
+        mret (mkst (Memory.update mem addr n) (incr_pc pc) loc ppc ploc)
+    end.
+  
+  (**  ------------------------------------------------------------------------- *)  
+  (** *** Helper functions for many-steps of evaluation *)
+
+  Fixpoint eval_until_pc (g : Cfg.t) (s : state)
+           (target_pc: pc)
+           (fuel : nat): err state :=
+    match fuel with
+    | 0 => raise "eval out of fuel"
+    | S n' =>
+      if (eq_dec_pc (st_pc s) target_pc) then mret s
+      else
+      's' <- (eval_step g s);
+      eval_until_pc g s' target_pc n'
+    end.
+
+  Definition eval_past_pc (g : Cfg.t) (s : state)
+             (target_pc : pc) (fuel : nat) : err state :=
+    's' <- eval_until_pc g s target_pc fuel;
+    eval_step g s'.
+
+  Definition eval_once_and_until_pc (g : Cfg.t) (s : state)
+             (target_pc: pc)
+             (fuel: nat) : err state :=
+    's' <- eval_step g s;
+    eval_until_pc g s' target_pc fuel.
+
+
+  (**  ------------------------------------------------------------------------- *)  
+  (** ** Correspondence between relational and executable definitions *)
+
+  (** Given that the relational and executable semantics share most of their "core"
+      functionality, it is pretty easy to prove that the two are equivalent.  
+   *)
+  
+  (** This tactic helps drive the evaluator by looking for a hypothesis that is 
+      "stuck" on a [trywith] because it can't be simplified without further case
+      analysis.  The tactic destructs the blocking expression, and is able to 
+      automatically discharge the goal by applying one of the [step] constructors,
+      which is provided as an argument.
+  *)
+  
+  Ltac eval_step_with_step next_state constructor_rule
+       cfg_well_formed fetched :=
+    match goal with
+    | H: match trywith _ ?X with _ => _ end = inr ?next_state |-
+      step ?cfg ?curr_state next_state =>
+      destruct X eqn:Heval;
+      inversion H;
+      eapply constructor_rule;
+      try rewrite Cfg.insn_at_pc_fetch;
+      try apply fetched;
+      try apply cfg_well_formed;
+      rewrite Heval;
+      reflexivity
+    | H : _ = inr next_state |-
+      step ?cfg ?curr_state next_state =>
+      inversion H;
+      eapply constructor_rule;
+      try rewrite Cfg.insn_at_pc_fetch;
+      try apply fetched;
+      try apply cfg_well_formed;
+      reflexivity
+    end.
+
+  Lemma evaluator_sound: forall g s s',
+      Cfg.wf_cfg g -> eval_step g s = inr s' -> step g s s'.
+  Proof.
+    intros g s s' wf_g; unfold eval_step;
+      destruct s as [mem curr_pc curr_loc previous_pc previous_loc];
+      destruct (Cfg.fetch g curr_pc) as 
+          [[uid [bop v1 v2 | pas | term | addr | addr v]] | ] eqn:fetched; simpl;
+      intros H;
+      [eval_step_with_step s' step_bop wf_g fetched |
+       eval_step_with_step s' step_phi wf_g fetched |
+       eval_step_with_step s' step_tmn wf_g fetched |
+       eval_step_with_step s' step_load wf_g fetched |
+       eval_step_with_step s' step_store wf_g fetched | inversion H].
+  Qed.
+  
+  Lemma evaluator_complete: forall g s s',
+      Cfg.wf_cfg g -> step g s s' -> eval_step g s = inr s'.
+  Proof.
+    intros g s s' wf_g step_rel; unfold eval_step;
+      inversion step_rel as
+        [mem pc loc bop v1 v2 uid n ppc ploc insn_at_pc_is eval_insn_ok s_eq s'_eq |
+         mem pc loc pas uid n ppc ploc insn_at_pc_is eval_insn_ok s_eq s'_eq |
+         mem pc label loc term uid ppc ploc insn_at_pc_is eval_insn_ok s_eq s'_eq |
+         mem pc loc uid addr ppc ploc insn_at_pc_is eval_insn_ok s'_eq |
+         mem pc loc uid addr v n ppc ploc insn_at_pc_is eval_insn_ok s_eq s'_eq];
+      simpl;
+    rewrite Cfg.insn_at_pc_fetch in insn_at_pc_is; try solve [apply wf_g];
+    try rewrite insn_at_pc_is; simpl;
+    try rewrite <- eval_insn_ok; try reflexivity.
+  Qed.
+  
+  Theorem evaluator_correct: forall g s s',
+      Cfg.wf_cfg g -> eval_step g s = inr s' <-> step g s s'.
+  Proof.
+    intros g s s' wf_g; split;
+      revert g s s' wf_g.
+    apply evaluator_sound.
+    apply evaluator_complete.
+  Qed.
+
+(** ------------------------------------------------------------------------- *)  
+(* ################################################################# *)
+(** * Determinism of [step] *)
+
+(** A direct consequence of the equivalence between the relational and 
+    functional specifications is that we can prove that [step] is 
+    deterministic.  
+
+    Note: one can prove that [step] is deterministic _without_ using the
+    correspondence with the evaluator, but it requires significantly more work!
+    It might be informative to try doing that proof. *)
+  
+Lemma step_deterministic : forall g s s1 s2, wf_cfg g ->
+  step g s s1 -> step g s s2 -> s1 = s2.
+Proof.
+  intros g s s1 s2 Hwfcfg Hs1 Hs2.
+  rewrite <- evaluator_correct in Hs1; auto.
+  rewrite <- evaluator_correct in Hs2; auto.
+  rewrite Hs1 in Hs2. inversion Hs2. reflexivity.
+Qed.
+
+
+  
+End Opsem.
+End Make.
+
+(**  ------------------------------------------------------------------------- *)  
+(* ================================================================= *)
+(** ** Instantiating the operational semantics to ListCFG *)
+
+(** For interesting applications of the operational semantics, such as building
+    a compiler or writing program transformations, we need to pick a concrete
+    representation of the CFG module.  For this development, we use the 
+    [ListCFG] definition.
+ *)
+
+Require Vminus.ListCFG.
+Module Import V := Make ListCFG.ListCFG.
+
+(**  ------------------------------------------------------------------------- *)  
