vminus/VminusStatics.v
@@ -1,0 +1,480 @@
+Require Import Arith.
+Require Import List.
+Import ListNotations.
+
+Require Import Vminus.Classes.
+Require Import Vminus.Util.
+Require Import Vminus.Env.
+Require Import Vminus.Vminus.
+Require Import Vminus.CFG.
+
+Require Import Vminus.Dom.
+Require Import Vminus.VminusOpSem.
+
+Module MakeStatics (Cfg: CFG).
+Import Cfg.
+
+(** * SSA Invariants: Typing CFGs*)
+
+(** The only ways in which a Vminus program can "go wrong" are
+    by accessing a local variable that hasn't been defined or jumping
+    to a label that isn't in the CFG.  Therefore, its "typing"
+    constraints ensure that each instruction only mentions local
+    identifiers that are in scope according to the domination
+    structure of the control-flow graph and that all mentioned labels
+    are associated with blocks defined in the CFG.  
+
+    These properties are partly enforced by the "syntactic"
+    well-formedness constraints imposed by the CFG interface (see
+    CFG.v), which ensure that labels and instruction identifiers are
+    unique.
+
+    To enforce the scoping property, we formalize the notion of
+    "dominance" in the control flow graph.  The module interface
+    [Dom.Spec] defines dominance for arbitrary graphs.  Here, we
+    instantiate the general theory with a suitable graph instance for
+    our CFGs.
+
+*)
+
+Module Typing.  
+(**  ------------------------------------------------------------------------- *)  
+(* ################################################################# *)
+(** * GRAPH instance for dominance calculation *)
+
+(** We need to define an graph instance that captures all the edges
+    of our CFGs.
+    
+    - vertices in the graph are just program points
+
+    - program points _within_ a single block have "fallthrough" edges determined by incrementing the program counter
+    
+    - a block [b1] terminated by a branch to [b2] induces an edge from [b1] to [b2] in the CFG.  
+  *)
+
+  
+  (** Graph edge relation *)
+
+  Inductive succ_pc (g:Cfg.t) : pc -> pc -> Prop :=
+  | succ_pc_S : forall p,
+      succ_pc g p (incr_pc p)
+  | succ_pc_J : forall p l i,
+      insn_at_pc g p i ->
+      In l (insn_lbls i) ->
+      succ_pc g p (block_entry l).
+
+(**  ------------------------------------------------------------------------- *)  
+(* ################################################################# *)
+(** * GRAPH instance for dominance calculation *)
+
+(** Graph of program points *)
+
+  Module PcGraph <: GRAPH.
+    Definition t := Cfg.t.
+    Definition V := pc.
+    Definition entry g := block_entry (entry_block g).
+    Definition Succ := succ_pc.
+    Definition Mem := wf_pc.
+  End PcGraph.
+
+(** Instantiate the dominance spec for this graph *)
+  
+  Module Export Dom := Dom.Spec PcGraph.
+
+  
+(**  ------------------------------------------------------------------------- *)  
+(* ################################################################# *)
+(** * Defining SSA scoping *)
+  
+(** We can now use the dominance properties of the CFG to define scoping
+    for well-formed SSA programs. We first need some auxliary predicates: *)
+
+(** The command at the given [pc] defines uid. *)
+
+  Definition def_at_pc (g:Cfg.t) (p:pc) (uid:uid) : Prop :=
+    exists c, insn_at_pc g p (uid, c) /\ defs_uid (uid, c). 
+
+  (** The [uid] has a definition that strictly dominates the pc [p]. *)
+ 
+  Definition uid_sdom_pc (g:Cfg.t) (uid:uid) (p:pc) : Prop :=
+    exists p', def_at_pc g p' uid /\ SDom g p' p.
+
+(**  ------------------------------------------------------------------------- *)  
+(* ----------------------------------------------------------------- *)
+(** *** Uses are dominated by their definitions *)
+  
+  (** All uses of a [uid] must be strictly dominated by
+      their definitions. However, we have to treat [phi] instructions
+      specially, since the "uses" of identifiers on the right-hand side of 
+      are conditioned on control flow.  
+
+      The right-hand-side of a phi node can safely refer to the identifier defined
+      by the phi node itself.  For example, consider this snippet of code:
+ [[
+      entry:
+        br blk      
+
+      blk: 
+        %x = phi [%entry: 0] [%blk: %x]    
+        br blk
+ ]]
+
+      For non-phi instructions, we simply require:
+  *)
+
+  Definition wf_use (g:Cfg.t) (i:insn) (p:pc) : Prop :=
+    ~is_phi i -> forall uid, In (val_uid uid) (insn_uses i) -> uid_sdom_pc g uid p.
+
+
+(**  ------------------------------------------------------------------------- *)  
+  (** *** Well-formed phi nodes *)
+
+  (**  Consider [ %x = phi [lbl1:v1, ...,lbln:vn] ].  This is well formed
+       when every predecessor block with terminator program point p' 
+       has a label associated with value v.  Moreover, if v is a uid then
+       the definition of the uid strictly dominates p' (i.e. the terminator
+       of the predecessor).
+  *)
+
+  Definition wf_phi_args (g:Cfg.t) (i:insn) (p:pc) : Prop :=
+    forall pred, succ_pc g pred (entry_of_pc p) ->
+      (exists v, In (lbl_of pred, v) (insn_phis i)) /\
+      (forall uid, In (lbl_of pred, val_uid uid) (insn_phis i) -> 
+          uid_sdom_pc g uid pred).
+
+  (** Moreover, we require that fore every labeled value appearing in the
+      right-hand side, there is a predecessor block with that label. *)
+  
+  Definition wf_phi_pred (g:Cfg.t) (i:insn) (p:pc) : Prop :=
+    forall l v, In (l, v) (insn_phis i) ->
+      (exists pred, succ_pc g pred (entry_of_pc p) /\ lbl_of pred = l).
+
+  Definition wf_phi (g:Cfg.t) (i:insn) (p:pc) : Prop :=
+    is_phi i -> wf_phi_args g i p
+             /\ wf_phi_pred g i p
+             /\ insn_phis i <> [].
+
+(**  ------------------------------------------------------------------------- *)  
+  (** *** Well-formed terminators *)
+
+  (** All jump targets must be legal block labels. *)  
+
+  Definition wf_lbl (g:Cfg.t) (i:insn) : Prop :=
+    forall l, In l (insn_lbls i) -> wf_pc g (block_entry l).
+
+
+  Definition reachable (g:Cfg.t) (p:pc) : Prop :=
+    exists path, Path g (block_entry (entry_block g)) p path.
+  
+(**  ------------------------------------------------------------------------- *)  
+(* ----------------------------------------------------------------- *)
+(** *** Well-formed instructions *)
+
+  Inductive wf_insn (g:Cfg.t) : insn -> pc -> Prop :=
+  | wf_insn_intro : forall i p
+      (Huse: wf_use g i p)
+      (Hlbl: wf_lbl g i)
+      (Hphi: wf_phi g i p)
+      (Hreach: reachable g p),
+      wf_insn g i p.
+
+  Inductive wf_prog (g:Cfg.t) : Prop :=
+  | wf_prog_intro : forall
+      (Hwfcfg : wf_cfg g)
+      (Hwfis : forall p i, insn_at_pc g p i -> wf_insn g i p)
+      (Hwftmn : forall p' i, tmn_pc g p' -> insn_at_pc g p' i -> is_tmn i)
+      (Hwfentry : forall p, ~ succ_pc g p (block_entry (entry_block g))),
+      wf_prog g.
+
+End Typing.
+
+(**  ------------------------------------------------------------------------- *)  
+(* ################################################################# *)
+(** * Type Safety *)
+
+(** We prove type safety for Vminus by setting up the usual _preservation_
+    and _progress_ theorems.  *)
+
+Module OpsemCorrect.
+  Module Import V := Make (Cfg).  
+  Import Typing Opsem.
+
+  
+
+
+  (** *** Dominance relation *)
+
+  (** A more convenient form for typing rules *)
+
+  Lemma uid_sdom_step : forall g uid' uid pc1 pc2 c,
+    wf_prog g ->
+    uid' <> uid ->
+    wf_pc g pc2 ->
+    succ_pc g pc1 pc2 ->
+    insn_at_pc g pc1 (uid, c) ->
+    uid_sdom_pc g uid' pc2 ->
+    uid_sdom_pc g uid' pc1.
+  Proof.
+    unfold uid_sdom_pc. 
+    intros g uid' uid pc1 pc2 c Hwff Hneq Hpc Hsucc Hi [pc' [Hdef Hdom]]. 
+    exists pc'. split. assumption. 
+    split. contradict Hneq. subst pc'.
+    inversion Hwff.
+    destruct Hdef as [? [? ?]]; eapply eq_pc_uid; eauto. 
+    inversion Hwff; eapply dom_step; eauto. 
+  Qed.
+
+  (** ** Progress & Preservation *)
+
+  (** Extend well-formedness definitions to include all components of 
+  the state. *)
+
+  Definition wf_loc (g:Cfg.t) (p:pc) (loc:loc) : Prop :=
+  forall uid, uid_sdom_pc g uid p -> exists n, loc uid = Some n.
+
+  Definition at_entry (g:Cfg.t) (p:pc) : Prop :=
+    entry_of_pc p = block_entry (entry_block g).
+
+  Inductive wf_state (g:Cfg.t) : state -> Prop :=
+  | wf_state_intro : forall st
+      (Hwfpc: wf_pc g st.(st_pc))
+      (Hwfloc: wf_loc g st.(st_pc) st.(st_loc))
+      (Hwfppc: at_entry g st.(st_pc) \/ 
+                 succ_pc g st.(st_ppc) (entry_of_pc st.(st_pc)))
+      (Hwfploc: at_entry g st.(st_pc) \/ 
+                  wf_loc g st.(st_ppc) st.(st_ploc)),
+      wf_state g st.
+
+  (** Initial state is well formed *)
+
+  Lemma wf_init_state : 
+    forall g m, wf_prog g ->
+    wf_state g (init_state g m).
+  Proof.
+    intros g m Hprog. inversion Hprog. 
+    apply wf_entry in Hwfcfg.
+    econstructor. auto.
+    red. simpl. intros. red in H. destruct H as [? [? [? ?]]].
+    red in H1. contradict H0.
+    cut (In x [block_entry (entry_block g)]). simpl. intuition.
+    eapply H1. econstructor. auto.
+    left. unfold init_state, at_entry, entry_of_pc. auto.
+    left. unfold init_state, at_entry, entry_of_pc. auto.
+  Qed.
+
+
+  (** *** Progress helper lemmas. *)
+
+  (** There are no phi nodes in the entry block. *)
+
+  Lemma at_entry_not_phi : forall g st i,
+    wf_prog g ->
+    at_entry g st.(st_pc) ->
+    insn_at_pc g st.(st_pc) i ->
+    ~ is_phi i.
+   Proof.
+     intros g st i Hprog Hentry Hinsn. 
+     destruct Hprog as [_ ? _ ?].
+
+     specialize (Hwfis _ _ Hinsn). inversion Hwfis; subst.
+     intro Hphi2. specialize (Hphi Hphi2). destruct Hphi as [H0 [H1 H2]].
+     destruct (insn_phis i) eqn:His. contradiction H2; auto.
+     assert (In p (insn_phis i)) as Hin. rewrite His. left; auto.
+     destruct p. apply H1 in Hin. destruct Hin as [pred [Hpred Ht0]].
+     specialize (Hwfentry pred). contradict Hwfentry. 
+     rewrite <- Hentry; auto.
+   Qed.
+
+  (** In a well-formed program with well-formed locals, evaluating
+  the values used by a non-phi instruction is never undefined. *)
+
+  Lemma eval_val__wf_loc : forall g pc loc i v,
+    wf_prog g ->
+    wf_loc g pc loc ->
+    ~is_phi i ->
+    insn_at_pc g pc i ->
+    In v (insn_uses i) ->
+    exists n, eval_val loc v = Some n.
+  Proof.
+    intros ? ? ? ? v Hwff Hwfloc Hnotphi Hi ?. 
+    destruct v as [uid | n].
+    simpl. inversion Hwff as [_ ? _]. apply Hwfis in Hi. 
+    destruct Hi as [? ? Huse].
+    destruct (is_phi_decidable i).
+    - contradiction.
+    specialize (Huse Hnotphi uid). 
+    lapply Huse; auto.
+    simpl; eauto.
+  Qed.
+
+  (** ** Progress *)
+
+  Definition FinalState (g:Cfg.t) (s:state) : Prop :=
+    exists uid, insn_at_pc g s.(st_pc) (uid, cmd_tmn tmn_ret).
+  
+  Lemma progress : forall g s,
+    wf_prog g -> wf_state g s ->
+    FinalState g s \/ exists s', step g s s'.
+  Proof.
+    intros g s Hwff Hwfs.
+    inversion Hwfs as [? Hwfpc]; subst. inversion Hwff.
+    pose proof (wf_pc_insn g Hwfcfg _ Hwfpc) as [[i c] Hi].
+    rename s into j. set (s:=j) in *. destruct j. 
+    destruct c.
+  
+    - (* Case "cmd_bop". *)
+    eelim (eval_val__wf_loc) with (v:=v) (loc:=st_loc0); eauto; simpl; auto.
+    eelim (eval_val__wf_loc) with (v:=v0) (loc:=st_loc0); eauto; simpl; auto.
+    intros n1 Heqn1 n2 Heqn2.
+    right. eexists. eapply step_bop; eauto. unfold eval_bop.
+    rewrite Heqn1, Heqn2. reflexivity. 
+
+    - (* Case "cmd_phi". *)
+    right. specialize (Hwfis _ _ Hi). inversion Hwfis; subst.
+    
+    destruct Hwfppc as [|Hwfppc]. 
+    exfalso; eapply at_entry_not_phi; eauto. simpl; trivial.
+    destruct Hwfploc as [|Hwfploc]. 
+    exfalso; eapply at_entry_not_phi; eauto. simpl; trivial.
+
+    destruct (Hphi I) as [Hphi2 _]. clear Hphi.
+    specialize (Hphi2 st_ppc0 Hwfppc). destruct Hphi2 as [[v Hin] Hdom].
+
+    cut (exists v, assoc Lbl.eq_dec (lbl_of st_ppc0) l = Some v). intros [v' Hv].
+    cut (exists n, eval_val st_ploc0 v' = Some n). intros [n Hn].
+    eexists. eapply step_phi. eauto. unfold eval_phi.
+    rewrite Hv. rewrite Hn. reflexivity.
+  
+    destruct v' as [i' | n']. simpl in *. apply Hwfploc. apply Hdom. 
+    eapply assoc_in. apply Hv. simpl; eauto.
+    eapply in_assoc_some. apply Hin.
+  
+    - (* Case "cmd_tmn". *)
+    destruct t0.
+    * (*  SCase "tmn_jmp". *)
+      right. eexists. eapply step_tmn. eauto. reflexivity.
+
+    * (* SCase "tmn_cbr". *)
+      cut (exists n, eval_val st_loc0 v = Some n). intros [n Heqn].
+      right. eexists. eapply step_tmn. eauto. simpl. rewrite Heqn. reflexivity.
+      eapply eval_val__wf_loc; eauto; simpl; auto. 
+
+    * (* SCase "tmn_ret". *)
+      left. unfold FinalState. eexists. eauto.
+
+    - (* Case "cmd_load". *)
+    right. eexists. apply step_load. eauto.
+
+    - (* Case "cmd_store". *)
+    right. cut (exists n1, eval_val st_loc0 v = Some n1). 
+    intros [n1 Heqn1]. eexists. eapply step_store. eauto. eauto.
+    eapply eval_val__wf_loc; eauto; simpl; auto.
+  Qed.
+
+  (** *** Some first steps towards preservation. *)
+
+  Lemma wf_pc_incr : forall g p i,
+    wf_prog g ->
+    wf_pc g p ->
+    insn_at_pc g p i ->
+    ~ is_tmn i ->
+    wf_pc g (incr_pc p).
+  Proof.
+    intros. inversion H. 
+    apply (wf_pc_tmn g Hwfcfg) in H0 as [pt [Ht Hle]].
+    eapply wf_pc_le_tmn; eauto.
+    inversion Hle; subst. destruct H0.
+    contradict H2. eapply Hwftmn; eauto. 
+    constructor; auto with arith.
+  Qed.
+
+  Lemma eval_tmn_in_lbls : forall l loc t uid,
+    Some l = eval_tmn loc t -> In l (insn_lbls (uid, cmd_tmn t)).
+  Proof.
+    intros.
+    destruct t0; simpl in *.
+    inversion H; auto.
+    destruct (eval_val loc v). injection H. 
+      destruct n; eauto.
+      discriminate H. discriminate H.
+  Qed.
+
+  (** *** More preservation helpers*)
+
+  Lemma not_def_sdom_step : forall g p1 p2 i uid,
+    wf_prog g ->
+    wf_pc g p2 ->
+    insn_at_pc g p1 i ->
+    ~ defs_uid i ->
+    succ_pc g p1 p2 ->
+    uid_sdom_pc g uid p2 ->
+    uid_sdom_pc g uid p1.
+  Proof. 
+    destruct i; intros. inversion H4 as [? [[? [? Ht]] ?]].
+    eapply uid_sdom_step; eauto. 
+    contradict Ht. subst t0. assert (x = p1). 
+    inversion H; eapply uid_at_pc_inj; try red; eauto. subst x.
+    replace (uid, x0) with (uid, c); trivial. 
+    inversion H; eapply insn_at_pc_func; eauto.
+  Qed.
+
+  Lemma wf_loc_succ : forall g p1 p2 loc uid n c,
+   wf_prog g ->
+   wf_pc g p2 ->
+   insn_at_pc g p1 (uid, c) ->
+   succ_pc g p1 p2 ->
+   wf_loc g p1 loc ->
+   wf_loc g p2 (update loc uid (Some n)).
+  Proof.
+    intros. red; intros. destruct (Uid.eq_dec uid0 uid). subst.
+    rewrite Locals.update_eq; eauto. reflexivity.
+    rewrite Locals.update_neq; eauto. apply H3.
+    eapply uid_sdom_step; eauto. 
+  Qed.
+
+  (** ** Preservation *)
+
+  Lemma preservation : forall g s s',
+    wf_prog g ->
+    wf_state g s -> step g s s' -> wf_state g s'.
+  Proof.
+    intros g _ s' Hwff [s Hwfpc Hwfloc] Hstep.
+    inversion Hstep; subst; simpl in *;
+      rename pc into pc0.
+    
+    - (* Case "step_bop". *)
+    assert (wf_pc g (incr_pc pc0)) as Hwfpc' by (eapply wf_pc_incr; eauto).
+    constructor; simpl; try solve [destruct pc0; auto].
+    eapply wf_loc_succ; eauto. constructor.
+
+    - (* Case "step_phi". *)
+    assert (wf_pc g (incr_pc pc0)) as Hwfpc' by (eapply wf_pc_incr; eauto).
+    constructor; simpl; try solve [destruct pc0; auto].
+    eapply wf_loc_succ; eauto. constructor.
+  
+    - (* Case "step_tmn". *)
+    assert (wf_pc g (l', 0)) as Hwfpc'.
+      inversion Hwff as [_ Hwfi _]. specialize (Hwfi _ _ H).
+      inversion Hwfi. red in Hlbl. apply Hlbl. 
+      eauto. eapply eval_tmn_in_lbls. eauto.
+
+    assert (succ_pc g pc0 (l', 0)) as Hsucc.
+      econstructor. eauto. eapply eval_tmn_in_lbls. eauto.
+    constructor; simpl; eauto. red; intros. apply Hwfloc.
+    eapply not_def_sdom_step; eauto.
+
+    - (* Case "step_load". *)
+    assert (wf_pc g (incr_pc pc0)) as Hwfpc' by (eapply wf_pc_incr; eauto).
+    constructor; simpl; try solve [destruct pc0; auto].
+    eapply wf_loc_succ; eauto. constructor.
+
+    - (* Case "step_store". *)
+    assert (wf_pc g (incr_pc pc0)) as Hwfpc' by (eapply wf_pc_incr; eauto).
+    constructor; simpl; try solve [destruct pc0; auto].
+    red; intros. apply Hwfloc. eapply not_def_sdom_step; eauto. constructor.
+  Qed.
+
+
+End OpsemCorrect.
+
+End MakeStatics.
